safe

Phi_System/PhiSem_Formalization_Tools.thy
@@ -1,5 +1,6 @@
-theory PhiSem_Formalization_To
+theory PhiSem_Formalization_Tools
   imports IDE_CP
+  keywords ":=" :: quasi_command
 begin
 
 section \<open>Tools for Formalizing Instructions\<close>
@@ -8,6 +9,10 @@ named_theorems discharging_semantic_debt
   \<open>Theorems that discharges or helps to discharge the debt axioms for semantic formalization.\<close>
 
 subsection \<open>Elementary Constructions for Formalizing Instructions\<close>
+
+definition \<open>semantic_literal = \<phi>arg\<close>
+
+ML \<open>Synchronized.change Phi_Syntax.semantic_oprs (Symtab.update (\<^const_name>\<open>semantic_literal\<close>, 0))\<close>
 
 definition \<phi>M_assert :: \<open>bool \<Rightarrow> unit proc\<close>
   where \<open>\<phi>M_assert P = (\<lambda>s. if P then Return \<phi>V_none s else {Invalid})\<close>
@@ -42,8 +47,9 @@ lemma Valid_Proc_\<phi>M_getV_raw[intro!, \<phi>reason 1200]:
   unfolding Valid_Proc_def \<phi>M_getV_raw_def
   by blast
 
+(*to depreciate the above!*)
 
-subsection \<open>Reasoning for Elementary Constructions\<close>
+subsection \<open>Basic Rules\<close>
 
 declare \<phi>SEQ[intro!]
 
@@ -51,6 +57,13 @@ lemma \<phi>M_assert[intro!]:
   \<open>(Inhabited X \<Longrightarrow> P) \<Longrightarrow> \<p>\<r>\<o>\<c> \<phi>M_assert P \<lbrace> X \<longmapsto> \<lambda>_. X \<rbrace> \<t>\<h>\<r>\<o>\<w>\<s> Any\<close>
   unfolding \<phi>M_assert_def
   by (rule \<phi>Inhabited; simp; rule)
+
+lemma semantic_assert_\<phi>app:
+  \<open> \<p>\<a>\<r>\<a>\<m> P
+\<Longrightarrow> \<p>\<r>\<e>\<m>\<i>\<s>\<e> P
+\<Longrightarrow> \<p>\<r>\<o>\<c> \<phi>M_assert P \<lbrace> X \<longmapsto> \<lambda>_. X \<rbrace>\<close>
+  unfolding \<phi>M_assert_def Premise_def
+  by (simp; rule)
 
 lemma \<phi>M_assert_True[simp]:
   \<open>\<phi>M_assert True = Return \<phi>V_none\<close>
@@ -70,6 +83,11 @@ lemma \<phi>M_assume1[intro!]:
   unfolding \<phi>M_assume_def \<phi>Procedure_def bind_def Return_def det_lift_def
   by clarsimp
 
+lemma semantic_assumption_\<phi>app:
+  \<open> \<p>\<a>\<r>\<a>\<m> P
+\<Longrightarrow> \<p>\<r>\<o>\<c> (\<phi>M_assume P) \<lbrace> Void \<longmapsto> Void \<s>\<u>\<b>\<j> P \<rbrace> \<close>
+  using \<phi>M_assume1 .
+
 lemma \<phi>M_tail_left:  \<open>\<p>\<r>\<o>\<c> F \<lbrace> 1\<heavy_comma> X \<longmapsto> Y \<rbrace> \<t>\<h>\<r>\<o>\<w>\<s> E \<Longrightarrow> \<p>\<r>\<o>\<c> F \<lbrace> X \<longmapsto> Y \<rbrace> \<t>\<h>\<r>\<o>\<w>\<s> E\<close> by simp
 lemma \<phi>M_tail_right: \<open>\<p>\<r>\<o>\<c> F \<lbrace> X \<longmapsto> \<lambda>v. 1 \<heavy_comma> Y v \<rbrace> \<t>\<h>\<r>\<o>\<w>\<s> E \<Longrightarrow> \<p>\<r>\<o>\<c> F \<lbrace> X \<longmapsto> Y \<rbrace> \<t>\<h>\<r>\<o>\<w>\<s> E\<close> by simp
 lemma \<phi>M_tail_right_right: \<open>\<p>\<r>\<o>\<c> F \<lbrace> X \<longmapsto> \<lambda>v. Y v\<heavy_comma> 1 \<rbrace> \<t>\<h>\<r>\<o>\<w>\<s> E \<Longrightarrow> \<p>\<r>\<o>\<c> F \<lbrace> X \<longmapsto> Y \<rbrace> \<t>\<h>\<r>\<o>\<w>\<s> E\<close> by simp
@@ -80,7 +98,7 @@ lemma \<phi>M_getV_raw[intro!]:
    \<open>(v \<Turnstile> (x \<Ztypecolon> A) \<Longrightarrow> \<p>\<r>\<o>\<c> F (VDT_dest v) \<lbrace> X \<longmapsto> Y \<rbrace> \<t>\<h>\<r>\<o>\<w>\<s> E  )
 \<Longrightarrow> \<p>\<r>\<o>\<c> \<phi>M_getV_raw VDT_dest (\<phi>arg v) F \<lbrace> X\<heavy_comma> x \<Ztypecolon> Val (\<phi>arg v) A \<longmapsto> Y \<rbrace> \<t>\<h>\<r>\<o>\<w>\<s> E \<close>
   unfolding \<phi>M_getV_raw_def Premise_def
-  by (clarsimp simp add: norm_precond_conj Val.unfold)
+  by (clarsimp simp add: Val.unfold norm_precond_conj)
 
 declare \<phi>M_getV_raw[where X=1, simplified, intro!]
 
@@ -98,1145 +116,150 @@ lemma \<phi>M_caseV[intro!]:
 \<Longrightarrow> \<p>\<r>\<o>\<c> \<phi>M_caseV F (\<phi>V_pair va vb) \<lbrace> X \<longmapsto> Y \<rbrace> \<t>\<h>\<r>\<o>\<w>\<s> E \<close>
   unfolding \<phi>M_caseV_def \<phi>V_pair_def by simp
 
-
-subsection \<open>Elementary Constructions for Reasoning Fictions\<close>
-
-text \<open>It is a Hybrid Dynamic Logic\<close>
-
-definition \<phi>Res_Spec :: \<open>rassn \<Rightarrow> rassn\<close>
-  where \<open>\<phi>Res_Spec S = RES.SPACE \<inter> S\<close>
-
-definition \<phi>Res_Sat  :: \<open>resource \<Rightarrow> rassn \<Rightarrow> bool\<close>
-  where \<open>\<phi>Res_Sat s P \<longleftrightarrow> s \<in> P\<close>
-
-abbreviation \<phi>Res_Sat'  :: \<open>resource \<Rightarrow> rassn \<Rightarrow> bool\<close> ("\<s>\<t>\<a>\<t>\<e> _ \<i>\<s> _" [11,11] 10)
-  where \<open>\<phi>Res_Sat' s P \<equiv> \<phi>Res_Sat s (\<phi>Res_Spec P)\<close>
-
-definition \<phi>Comp_Sat :: \<open>'ret comp set \<Rightarrow> ('ret \<phi>arg \<Rightarrow> rassn) \<Rightarrow> (ABNM \<Rightarrow> rassn) \<Rightarrow> bool\<close>
-  where \<open>\<phi>Comp_Sat c S E \<longleftrightarrow> c \<subseteq> LooseState S E\<close>
-
-abbreviation \<phi>Comp_Sat' :: \<open>'ret comp set \<Rightarrow> ('ret \<phi>arg \<Rightarrow> rassn) \<Rightarrow> (ABNM \<Rightarrow> rassn) \<Rightarrow> bool\<close>
-                          ("_ \<r>\<e>\<s>\<u>\<l>\<t>\<s> \<i>\<n> _ \<t>\<h>\<r>\<o>\<w>\<s> _" [11,11,11] 10)
-  where \<open>\<phi>Comp_Sat' c S E \<equiv> \<phi>Comp_Sat c (\<lambda>r. \<phi>Res_Spec (S r)) (\<lambda>e. \<phi>Res_Spec (E e))\<close>
-
-lemma \<phi>Comp_Sat_success[simp]:
-  \<open> ({Success ret res} \<r>\<e>\<s>\<u>\<l>\<t>\<s> \<i>\<n> Y \<t>\<h>\<r>\<o>\<w>\<s> E)
-\<longleftrightarrow> (\<s>\<t>\<a>\<t>\<e> res \<i>\<s> Y ret)\<close>
-  unfolding \<phi>Comp_Sat_def \<phi>Res_Sat_def by simp
-
-lemma \<phi>Res_Sat_0[iff]:
-  \<open>\<not> (\<s>\<t>\<a>\<t>\<e> x \<i>\<s> {})\<close> \<open>\<not> (\<s>\<t>\<a>\<t>\<e> x \<i>\<s> 0)\<close>
-  unfolding \<phi>Res_Sat_def \<phi>Res_Spec_def by (simp add: zero_set_def)+
-
-(*lemma \<phi>Res_Sat_0[iff]:
-  \<open>(\<s>\<t>\<a>\<t>\<e> x \<i>\<s> {})\<close> \<open>\<not> (\<s>\<t>\<a>\<t>\<e> x \<i>\<s> 0)\<close>
-  unfolding \<phi>Res_Sat_def by (simp add: zero_set_def)+
-
-lemma \<phi>Res_Spec_1[iff]:
-  \<open>\<phi>Res_Spec 1 = 1\<close>
-  unfolding \<phi>Res_Spec_def by (simp add: set_eq_iff; blast) *)
-
-(*lemma \<phi>Res_Spec_mult_homo:
-  \<open>\<phi>Res_Spec (A * B) = \<phi>Res_Spec A * \<phi>Res_Spec B\<close>
-  unfolding \<phi>Res_Spec_def
-  by (clarsimp simp add: set_eq_iff times_set_def; rule; clarsimp simp add: RES.SPACE_mult_homo; blast) *)
-
-lemma \<phi>Res_Sat_subj[iff]:
-  \<open>(\<s>\<t>\<a>\<t>\<e> s \<i>\<s> S \<s>\<u>\<b>\<j> P) \<longleftrightarrow> (\<s>\<t>\<a>\<t>\<e> s \<i>\<s> S) \<and> P\<close>
-  unfolding \<phi>Res_Sat_def \<phi>Res_Spec_def by (simp add: Subjection_expn_set set_eq_iff)
-
-lemma \<phi>Comp_Sat_subj:
-  \<open> P
-\<Longrightarrow> c \<r>\<e>\<s>\<u>\<l>\<t>\<s> \<i>\<n> S \<t>\<h>\<r>\<o>\<w>\<s> E
-\<Longrightarrow> c \<r>\<e>\<s>\<u>\<l>\<t>\<s> \<i>\<n> (\<lambda>v. S v \<s>\<u>\<b>\<j> P) \<t>\<h>\<r>\<o>\<w>\<s> E\<close>
-  by (clarsimp simp add: set_eq_iff)
-
-lemma \<phi>Res_Sat_ex[iff]:
-  \<open>(\<s>\<t>\<a>\<t>\<e> s \<i>\<s> ExSet S) \<longleftrightarrow> (\<exists>x. \<s>\<t>\<a>\<t>\<e> s \<i>\<s> S x)\<close>
-  unfolding \<phi>Res_Sat_def \<phi>Res_Spec_def by (simp add: ExSet_expn_set set_eq_iff)
-
-lemma \<phi>Res_Sat_ex_ret:
-  \<open> c \<r>\<e>\<s>\<u>\<l>\<t>\<s> \<i>\<n> S x \<t>\<h>\<r>\<o>\<w>\<s> E
-\<Longrightarrow> c \<r>\<e>\<s>\<u>\<l>\<t>\<s> \<i>\<n> (\<lambda>v. \<exists>*x. S x v) \<t>\<h>\<r>\<o>\<w>\<s> E\<close>
-  unfolding \<phi>Comp_Sat_def \<phi>Res_Spec_def
-  apply (clarsimp simp add: ExSet_expn_set set_eq_iff subset_iff)
-  subgoal for x by (cases x; clarsimp simp add: ExSet_expn_set set_eq_iff subset_iff; blast) .
-
-lemma \<phi>Res_Sat_ex_abn:
-  \<open> c \<r>\<e>\<s>\<u>\<l>\<t>\<s> \<i>\<n> S \<t>\<h>\<r>\<o>\<w>\<s> E x
-\<Longrightarrow> c \<r>\<e>\<s>\<u>\<l>\<t>\<s> \<i>\<n> S \<t>\<h>\<r>\<o>\<w>\<s> (\<lambda>v. \<exists>*x. E x v)\<close>
-  unfolding \<phi>Comp_Sat_def \<phi>Res_Spec_def
-  apply (clarsimp simp add: ExSet_expn_set set_eq_iff subset_iff)
-  subgoal for x by (cases x; clarsimp simp add: ExSet_expn_set set_eq_iff subset_iff; blast) .
-
-(*lemma \<phi>INTERP_RES_\<phi>Res_Spec:
-  \<open>res \<in> INTERP_RES fic \<longleftrightarrow> res \<in> \<phi>Res_Spec (\<I> FIC.INTERP fic) \<and> fic \<in> FIC.SPACE\<close>
-  unfolding In_INTERP_RES \<phi>Res_Spec_def by simp blast *)
-
-term \<open>\<s>\<t>\<a>\<t>\<e> s \<i>\<s> FIC.INTERP (r * p) \<s>\<u>\<b>\<j> p. p \<in> P \<and> r \<in> FIC.SPACE \<and> p \<in> FIC.SPACE \<and> r ## p\<close>
-
-lemma \<phi>Procedure_Hybrid_DL:
-  \<open> \<p>\<r>\<o>\<c> f \<lbrace> P \<longmapsto> Q \<rbrace> \<t>\<h>\<r>\<o>\<w>\<s> E
-\<longleftrightarrow> (\<forall>r s. (\<s>\<t>\<a>\<t>\<e> s \<i>\<s> FIC.INTERP (r * p) \<s>\<u>\<b>\<j> p. p \<in> P \<and> r \<in> FIC.SPACE \<and> p \<in> FIC.SPACE \<and> r ## p)
-       \<longrightarrow> (f s \<r>\<e>\<s>\<u>\<l>\<t>\<s> \<i>\<n> (\<lambda>v. FIC.INTERP (r * q) \<s>\<u>\<b>\<j> q. q \<in> Q v \<and> r \<in> FIC.SPACE \<and> q \<in> FIC.SPACE \<and> r ## q)
-                \<t>\<h>\<r>\<o>\<w>\<s> (\<lambda>v. FIC.INTERP (r * e) \<s>\<u>\<b>\<j> e. e \<in> E v \<and> r \<in> FIC.SPACE \<and> e \<in> FIC.SPACE \<and> r ## e)))\<close>
-  apply rule
-   apply (unfold \<phi>Procedure_alt INTERP_SPEC \<phi>Res_Sat_def \<phi>Comp_Sat_def \<phi>Res_Spec_def subset_iff)
-   apply (clarsimp simp add: times_set_def ExSet_expn_set Subjection_expn_set In_INTERP_RES)
-  thm In_INTERP_RES
-  subgoal premises prems for r res s c proof-
-    have t1: \<open>(\<exists>fic. (\<exists>y. fic = r * y \<and> y \<in> P \<and> r ## y) \<and> res \<in> RES.SPACE \<and> fic \<in> FIC.SPACE \<and> res \<in> FIC.INTERP fic)\<close>
-      using FIC.SPACE_mult_homo prems by blast
-    show ?thesis
-      apply (insert prems(1)[THEN spec[where x=res], THEN spec[where x=r], THEN mp, OF t1,
-              THEN spec[where x=s], THEN mp, OF \<open>s \<in> f res\<close>])
-      apply (cases s; clarsimp simp add: ExSet_expn_set Subjection_expn_set INTERP_SPEC In_INTERP_RES FIC.SPACE_mult_homo)
-      apply force
-      using FIC.SPACE_mult_homo by blast
-  qed
-  apply (clarsimp simp add: times_set_def ExSet_expn_set Subjection_expn_set In_INTERP_RES)
-  subgoal premises prems for res r s c proof-
-    have t1: \<open>res \<in> RES.SPACE \<and> (\<exists>c. res \<in> FIC.INTERP (r * c) \<and> c \<in> P \<and> r \<in> FIC.SPACE \<and> c \<in> FIC.SPACE \<and> r ## c)\<close>
-      using prems FIC.SPACE_mult_homo by blast
-    show ?thesis
-      apply (insert prems(1)[THEN spec[where x=r], THEN spec[where x=res], THEN mp, OF t1,
-              THEN spec[where x=s], THEN mp, OF \<open>s \<in> _\<close>])
-      apply (cases s; simp add: ExSet_expn_set Subjection_expn_set INTERP_SPEC In_INTERP_RES)
-      using FIC.SPACE_mult_homo apply blas
-      using FIC.SPACE_mult_homo by blas
-  qed .
-
-lemma \<phi>Res_Spec_expn_R:
-  \<open>\<phi>Res_Spec (FIC.INTERP (r * p) \<s>\<u>\<b>\<j> p. p \<in> (R \<heavy_comma> X) \<and> r \<in> FIC.SPACE \<and> p \<in> FIC.SPACE \<and> r ## p)
- = \<phi>Res_Spec (FIC.INTERP (r * u * x) \<s>\<u>\<b>\<j> u x. u \<in> R \<and> x \<in> X \<and> (r * u) \<in> FIC.SPACE \<and> x \<in> FIC.SPACE
-                                           \<and> r ## u \<and> (r * u) ## x)\<close>
-  unfolding set_eq_iff \<phi>Res_Spec_def
-  apply (clarsimp simp add: ExSet_expn_set Subjection_expn_set INTERP_SPEC set_mult_expn; rule; clarify)
-  apply (metis FIC.SPACE_mult_homo sep_disj_multD1 sep_disj_multI1 sep_mult_assoc')
-  by (metis FIC.SPACE_mult_homo sep_disj_multD2 sep_disj_multI2 sep_mult_assoc)
-
-(*
-lemma \<phi>Res_Sat_expn_R:
-  \<open> (\<s>\<t>\<a>\<t>\<e> s \<i>\<s> \<I> FIC.INTERP (r * p) \<s>\<u>\<b>\<j> p. p \<in> (R \<heavy_comma> X) \<and> r \<in> FIC.SPACE \<and> p \<in> FIC.SPACE \<and> r ## p)
-\<longleftrightarrow> (\<s>\<t>\<a>\<t>\<e> s \<i>\<s> \<I> FIC.INTERP (r * u * x) \<s>\<u>\<b>\<j> u x. u \<in> R \<and> x \<in> X \<and> (r * u) \<in> FIC.SPACE \<and> x \<in> FIC.SPACE
-                                           \<and> r ## u \<and> (r * u) ## x)\<close>
-  unfolding \<phi>Res_Sat_def using \<phi>Res_Spec_expn_R by simp *)
-
-(*lemma \<phi>Res_Comp_expn_R:
-  \<open> (c \<r>\<e>\<s>\<u>\<l>\<t>\<s> \<i>\<n> \<I> FIC.INTERP (r * p) \<s>\<u>\<b>\<j> p. p \<in> (R \<heavy_comma> X) \<and> r \<in> FIC.SPACE \<and> p \<in> FIC.SPACE \<and> r ## p)
-\<longleftrightarrow> (c \<r>\<e>\<s>\<u>\<l>\<t>\<s> \<i>\<n> \<I> FIC.INTERP (r * u * x) \<s>\<u>\<b>\<j> u x. u \<in> R \<and> x \<in> X \<and> (r * u) \<in> FIC.SPACE \<and> x \<in> FIC.SPACE
-                                           \<and> r ## u \<and> (r * u) ## x)\<close>
-  unfolding \<phi>Res_Sat_def using \<phi>Res_Spec_expn_R by simp *)
-
-
-lemma \<phi>Res_Sat_expn_impEx:
-  \<open>((\<s>\<t>\<a>\<t>\<e> s \<i>\<s> (ExSet A)) \<longrightarrow> P) \<longleftrightarrow> (\<forall>a. (\<s>\<t>\<a>\<t>\<e> s \<i>\<s> A a) \<longrightarrow> P)\<close>
-  by (simp add: ExSet_def \<phi>Res_Sat_def \<phi>Res_Spec_def)
-
-lemma \<phi>Res_Sat_expn_impSubj:
-  \<open>((\<s>\<t>\<a>\<t>\<e> s \<i>\<s> A \<s>\<u>\<b>\<j> B) \<longrightarrow> P) \<longleftrightarrow> (B \<longrightarrow> (\<s>\<t>\<a>\<t>\<e> s \<i>\<s> A) \<longrightarrow> P)\<close>
-  by (simp add: Subjection_expn_set \<phi>Res_Sat_def \<phi>Res_Spec_def; blast)
-
-
-paragraph \<open>Weakest Precondition Transformer for \<phi>Res_Spec\<close>
-
-lemma \<phi>M_RS_WP_SEQ[intro!]:
-  \<open> F s \<r>\<e>\<s>\<u>\<l>\<t>\<s> \<i>\<n> P \<t>\<h>\<r>\<o>\<w>\<s> E
-\<Longrightarrow> (\<And>v s. \<s>\<t>\<a>\<t>\<e> s \<i>\<s> P v \<Longrightarrow> G v s \<r>\<e>\<s>\<u>\<l>\<t>\<s> \<i>\<n> Q \<t>\<h>\<r>\<o>\<w>\<s> E)
-\<Longrightarrow> (F \<bind> G) s \<r>\<e>\<s>\<u>\<l>\<t>\<s> \<i>\<n> Q \<t>\<h>\<r>\<o>\<w>\<s> E\<close>
-  unfolding bind_def subset_iff \<phi>Res_Sat_def \<phi>Comp_Sat_def
-  apply clarsimp subgoal for s s'
-    by (cases s'; simp; cases s; clarsimp ; blast) .
-
-
-section \<open>Predefined Resource Snippet\<close>
-
-subsection \<open>Resource Base\<close>
-
-locale resource =
-  resource_kind RES.DOMAIN Res
-  for Res :: "'T::sep_algebra resource_entry"
-begin
-
-lemma get_res_valid_raw:
-  \<open> res \<in> RES.SPACE
-\<Longrightarrow> get res \<in>\<^sub>S\<^sub>H domain\<close>
-  unfolding RES.SPACE_def
-  by (simp, metis in_DOMAIN proj_inj)
-
-lemma get_res_Valid:
-  \<open> \<s>\<t>\<a>\<t>\<e> res \<i>\<s> S
-\<Longrightarrow> get res \<in>\<^sub>S\<^sub>H domain\<close>
-  unfolding \<phi>Res_Spec_def \<phi>Res_Sat_def by (clarsimp simp add: \<r>_valid_split')
-
-definition \<open>basic_fiction = (\<lambda>x. { 1(Res #= x) })\<close>
-
-lemma basic_fiction_homo_one[simp]:
-  \<open>homo_one basic_fiction\<close>
-  unfolding homo_one_def basic_fiction_def by (clarsimp simp add: set_eq_iff)
-
-lemma \<F>_itself_expn[\<phi>expns]:
-  \<open>R2 ## x
-\<Longrightarrow> \<phi>Res_Spec ((basic_fiction \<Zcomp>\<^sub>\<I> \<F>_it) (R2 * x))
-  = \<phi>Res_Spec ((basic_fiction \<Zcomp>\<^sub>\<I> \<F>_it) R2 * {mk x})\<close>
-  unfolding \<phi>Res_Spec_def set_eq_iff
-  apply (clarsimp simp add: set_mult_expn basic_fiction_def prj.homo_mult)
-  apply (rule; clarify)
-   apply (simp add: mk_homo_mult sep_mult_assoc')
-  using SPACE_mult_homo inj.homo_mult by force
-
-lemma implies_part:
-  \<open> \<s>\<t>\<a>\<t>\<e> res \<i>\<s> R * {mk x}
-\<Longrightarrow> x \<preceq>\<^sub>S\<^sub>L get res\<close>
-  unfolding \<phi>Res_Sat_def \<phi>Res_Spec_def join_sub_def times_set_def apply clarsimp
-  using get_homo_mult sep_disj_get_name by fastforce
-
-end
-
-
-subsection \<open>Fictions\<close>
-
-subsubsection \<open>Fiction Base\<close>
-
-locale basic_fiction =
-   R: resource Res
-+  fiction_kind FIC.DOMAIN INTERPRET Fic \<open>R.basic_fiction \<Zcomp>\<^sub>\<I> I\<close>
-for Res :: "'T::sep_algebra resource_entry"
-and I :: "('U::sep_algebra, 'T) interp"
-and Fic :: "'U fiction_entry"
-begin
-
-paragraph \<open>\<phi>-Type\<close>
-
-definition \<phi> :: \<open>('U, 'x) \<phi> \<Rightarrow> (fiction, 'x) \<phi>\<close>
-    \<comment> \<open>\<phi>Type for level-1 mapping\<close>
-  where \<open>\<phi> T = (\<lambda>x. { mk v |v. v \<Turnstile> (x \<Ztypecolon> T) })\<close>
-
-lemma \<phi>_expn[simp, \<phi>expns]:
-  \<open>p \<Turnstile> (x \<Ztypecolon> \<phi> T) \<longleftrightarrow> (\<exists>v. p = mk v \<and> v \<Turnstile> (x \<Ztypecolon> T))\<close>
-  unfolding \<phi>Type_def \<phi>_def Satisfaction_def by simp
-
-lemma \<phi>_inhabited[elim!]:
-  \<open>Inhabited (x \<Ztypecolon> \<phi> T) \<Longrightarrow> (Inhabited (x \<Ztypecolon> T) \<Longrightarrow> C) \<Longrightarrow> C\<close>
-  unfolding Inhabited_def by simp
-
-lemma [\<phi>inhabitance_rule 1000]:
-  \<open> x \<Ztypecolon> T \<i>\<m>\<p>\<l>\<i>\<e>\<s> C
-\<Longrightarrow> x \<Ztypecolon> \<phi> T \<i>\<m>\<p>\<l>\<i>\<e>\<s> C\<close>
-  unfolding Inhabited_def by simp
-
-lemma \<phi>_Prod:
-  \<open> \<phi> T \<^emph> \<phi> U = \<phi> (T \<^emph> U)\<close>
-  apply (rule \<phi>Type_eqI; clarsimp; rule; clarsimp)
-  apply (metis mk_homo_mult)
-  by (metis fun_1upd_homo inj.homo_mult sep_disj_mk)
-
-lemma \<phi>_\<phi>None:
-  \<open>\<phi> \<circle> = \<circle>\<close>
-  by (rule \<phi>Type_eqI; simp)
-
-lemma \<phi>_unit:
-  \<open>(1 \<Ztypecolon> \<phi> Itself) = Void\<close>
-  by (clarsimp simp add: BI_eq_iff)
-
-
-lemma [\<phi>reason 1200 for \<open>(?x \<Ztypecolon> \<phi> \<circle>) = ?Z @action clean_automation_waste\<close>]:
-  \<open>(x \<Ztypecolon> \<phi> \<circle>) = (() \<Ztypecolon> \<circle>) @action clean_automation_waste\<close>
-  unfolding Action_Tag_def \<phi>_\<phi>None by simp
-
-lemma [\<phi>reason 1300 for \<open>(?x \<Ztypecolon> \<phi> \<circle>) = ?Z @action clean_automation_waste\<close>]:
-  \<open>(x \<Ztypecolon> \<phi> \<circle>) = 1 @action clean_automation_waste\<close>
-  unfolding Action_Tag_def \<phi>_\<phi>None by simp
-
-
-(*
-lemma [\<phi>reason 1500 for \<open>(x \<Ztypecolon> \<phi> \<circle>) \<t>\<r>\<a>\<n>\<s>\<f>\<o>\<r>\<m>\<s> ?Y \<w>\<i>\<t>\<h> ?P @action (?Act::?'act::simplification action)\<close>]:
-  \<open>(x \<Ztypecolon> \<phi> \<circle>) \<t>\<r>\<a>\<n>\<s>\<f>\<o>\<r>\<m>\<s> (() \<Ztypecolon> \<circle>) @action Act\<close>
-  for Act :: \<open>'act::simplification action\<close>
-  unfolding Action_Tag_def \<phi>_\<phi>None
-  by (simp add: transformation_refl) *)
-
-paragraph \<open>Reasoning Rules\<close>
-
-lemma \<phi>_cast[\<phi>reason add]:
-  \<open> x \<Ztypecolon> T \<t>\<r>\<a>\<n>\<s>\<f>\<o>\<r>\<m>\<s> y \<Ztypecolon> U \<w>\<i>\<t>\<h> P
-\<Longrightarrow> x \<Ztypecolon> \<phi> T \<t>\<r>\<a>\<n>\<s>\<f>\<o>\<r>\<m>\<s> y \<Ztypecolon> \<phi> U \<w>\<i>\<t>\<h> P\<close>
-  unfolding Transformation_def by clarsimp
-
-lemma \<phi>_Structural_Extract:
-  \<open> x \<Ztypecolon> T \<^emph> W \<t>\<r>\<a>\<n>\<s>\<f>\<o>\<r>\<m>\<s> y \<Ztypecolon> U \<^emph> R \<w>\<i>\<t>\<h> P @action \<A>SE True
-\<Longrightarrow> x \<Ztypecolon> \<phi> T \<^emph> \<phi> W \<t>\<r>\<a>\<n>\<s>\<f>\<o>\<r>\<m>\<s> y \<Ztypecolon> \<phi> U \<^emph> \<phi> R \<w>\<i>\<t>\<h> P @action \<A>SE True\<close>
-  unfolding Action_Tag_def
-  by (simp add: \<phi>Prod_expn'[symmetric] \<phi>_Prod \<phi>_cast)
-
-declare \<phi>_Structural_Extract[(*THEN SE_clean_waste,*) \<phi>reason 1200]
-
-(* TODO!!!!
-lemma [(*THEN SE_clean_waste',*) \<phi>reason 1211]:
-  \<open> x \<Ztypecolon> T \<^emph> W \<t>\<r>\<a>\<n>\<s>\<f>\<o>\<r>\<m>\<s> y \<Ztypecolon> U \<^emph> R \<w>\<i>\<t>\<h>
-      (Reverse_Transformation RP (y' \<Ztypecolon> U' \<^emph> R' \<t>\<r>\<a>\<n>\<s>\<f>\<o>\<r>\<m>\<s> x' \<Ztypecolon> T' \<^emph> W' \<w>\<i>\<t>\<h> P') \<and> P) @action \<A>SE True
-\<Longrightarrow> x \<Ztypecolon> \<phi> T \<^emph> \<phi> W \<t>\<r>\<a>\<n>\<s>\<f>\<o>\<r>\<m>\<s> y \<Ztypecolon> \<phi> U \<^emph> \<phi> R \<w>\<i>\<t>\<h>
-      (Reverse_Transformation RP (y' \<Ztypecolon> \<phi> U' \<^emph> \<phi> R' \<t>\<r>\<a>\<n>\<s>\<f>\<o>\<r>\<m>\<s> x' \<Ztypecolon> \<phi> T' \<^emph> \<phi> W' \<w>\<i>\<t>\<h> P') \<and> P) @action \<A>SE True\<close>
-  unfolding Generated_Rule_def Action_Tag_def
-  by (rule transformation_weaken, defer_tac,
-      rule \<phi>_Structural_Extract[unfolded Action_Tag_def], assumption,
-      clarify, rule \<phi>_Structural_Extract[unfolded Action_Tag_def], blast)*)
-
-(*
-lemma [\<phi>reason 1100]:
-  \<open> Structure_Info T P
-\<Longrightarrow> Structure_Info (\<phi> T) P\<close>
-  unfolding Structure_Info_def
-  by blast *)
-
-(* TODO!!!!
-declare NToA_by_structural_extraction
-    [where T=\<open>\<phi> T\<close> and U=\<open>\<phi> U\<close> for T U,
-     \<phi>reason 80 if \<open>PLPR_Env.boolean_flag \<^const_name>\<open>ToA_flag_deep\<close> true o fst\<close>]
-
-declare NToA_by_structural_extraction__reverse_transformation
-    [where T=\<open>\<phi> T\<close> and U=\<open>\<phi> U\<close> and T'=\<open>\<phi> T'\<close> and U'=\<open>\<phi> U'\<close> for T T' U U',
-     \<phi>reason 83 if \<open>PLPR_Env.boolean_flag \<^const_name>\<open>ToA_flag_deep\<close> true o fst\<close>]
-*)
-
-(*lemma NToA_by_structural_extraction:
-  " Structure_Info U Q
-\<Longrightarrow> \<s>\<i>\<m>\<p>\<l>\<i>\<f>\<y> Q' : Q
-\<Longrightarrow> (Q' \<Longrightarrow> Try Any (Structural_Extract (y \<Ztypecolon> \<phi> U) R1 (x \<Ztypecolon> \<phi> T) W P2))
-\<Longrightarrow> A \<t>\<r>\<a>\<n>\<s>\<f>\<o>\<r>\<m>\<s> R2 \<heavy_comma> \<blangle> W \<brangle> \<w>\<i>\<t>\<h> P1
-\<Longrightarrow> A \<heavy_comma> y \<Ztypecolon> \<phi> U \<t>\<r>\<a>\<n>\<s>\<f>\<o>\<r>\<m>\<s> R2\<heavy_comma> R1\<heavy_comma> \<blangle> x \<Ztypecolon> \<phi> T \<brangle> \<w>\<i>\<t>\<h> P1 \<and> P2"
-  unfolding Premise_def FOCUS_TAG_def Structural_Extract_def Simplify_def Try_def
-  \<medium_left_bracket> premises SI and Q and SE and A
-  have \<open>Q'\<close> using \<phi> SI[unfolded Structure_Info_def] Q by blast
-  ;;  A[THEN transformation_right_frame]
-     SE[OF \<open>Q'\<close>]
-  \<medium_right_bracket> certified using \<phi> by simp .
-
-lemma NToA_by_structural_extraction__reverse_transformation:
-  " Structure_Info U Q
-\<Longrightarrow> \<s>\<i>\<m>\<p>\<l>\<i>\<f>\<y> Q' : Q
-\<Longrightarrow> (Q' \<Longrightarrow> Try Any (Structural_Extract (y \<Ztypecolon> \<phi> U) R1 (x \<Ztypecolon> \<phi> T) W
-             (Reverse_Transformation RP2 (Structural_Extract (x' \<Ztypecolon> \<phi> T') W' (y' \<Ztypecolon> \<phi> U') R1' P2') \<and> P2)))
-\<Longrightarrow> A \<t>\<r>\<a>\<n>\<s>\<f>\<o>\<r>\<m>\<s> R2 \<heavy_comma> \<blangle> W \<brangle> \<w>\<i>\<t>\<h> (Reverse_Transformation RP1 (R2'\<heavy_comma> \<blangle> W' \<brangle> \<t>\<r>\<a>\<n>\<s>\<f>\<o>\<r>\<m>\<s> A' \<w>\<i>\<t>\<h> P1') \<and> P1)
-\<Longrightarrow> A \<heavy_comma> y \<Ztypecolon> \<phi> U \<t>\<r>\<a>\<n>\<s>\<f>\<o>\<r>\<m>\<s> R2\<heavy_comma> R1\<heavy_comma> \<blangle> x \<Ztypecolon> \<phi> T \<brangle> \<w>\<i>\<t>\<h>
-      (Reverse_Transformation (RP2 \<and>\<^sub>\<r> RP1) (R2'\<heavy_comma> R1'\<heavy_comma> \<blangle> x' \<Ztypecolon> \<phi> T' \<brangle> \<t>\<r>\<a>\<n>\<s>\<f>\<o>\<r>\<m>\<s> A'\<heavy_comma> y' \<Ztypecolon> \<phi> U' \<w>\<i>\<t>\<h> P1' \<and> P2')
-          \<and> P1 \<and> P2)"
-  unfolding Premise_def FOCUS_TAG_def Structural_Extract_def Simplify_def
-            Generated_Rule_def Compact_Antecedent_def Try_def
-  \<medium_left_bracket> premises SI and Q and SE and A
-  have \<open>Q'\<close> using \<phi> SI[unfolded Structure_Info_def] Q by blast
-  ;; A[THEN transformation_right_frame]
-     SE[OF \<open>Q'\<close>]
-  \<medium_right_bracket> certified apply  (simp add: \<phi>)
-  \<medium_left_bracket>
-    have A : \<open>R2' \<heavy_comma> W' \<t>\<r>\<a>\<n>\<s>\<f>\<o>\<r>\<m>\<s> A' \<w>\<i>\<t>\<h> P1'\<close> using \<phi>_previous \<open>RP2 \<and> RP1\<close> by simp
-    have SE: \<open>(R1' \<heavy_comma> x' \<Ztypecolon> \<phi> T' \<t>\<r>\<a>\<n>\<s>\<f>\<o>\<r>\<m>\<s> W' \<heavy_comma> y' \<Ztypecolon> \<phi> U' \<w>\<i>\<t>\<h> P2')\<close> using \<phi>_previous \<open>RP2 \<and> RP1\<close> by simp
-    ;; SE A[THEN transformation_right_frame]
-  \<medium_right_bracket>. .
-*)
-
-lemma NToA_skip [\<phi>reason 1200 except \<open> _ \<heavy_comma> ?y \<Ztypecolon> \<phi> ?U \<t>\<r>\<a>\<n>\<s>\<f>\<o>\<r>\<m>\<s> _ \<heavy_comma> \<blangle> ?x \<Ztypecolon> \<phi> ?T \<brangle> \<w>\<i>\<t>\<h> _\<close> ]:
-  " R \<t>\<r>\<a>\<n>\<s>\<f>\<o>\<r>\<m>\<s> R'\<heavy_comma> \<blangle> x \<Ztypecolon> \<phi> T \<brangle> \<w>\<i>\<t>\<h> P
-\<Longrightarrow> R \<heavy_comma> X \<t>\<r>\<a>\<n>\<s>\<f>\<o>\<r>\<m>\<s> R'\<heavy_comma> X\<heavy_comma> \<blangle> x \<Ztypecolon> \<phi> T \<brangle> \<w>\<i>\<t>\<h> P"
-  unfolding Action_Tag_def FOCUS_TAG_def split_paired_All Action_Tag_def
-  by (metis ab_semigroup_mult_class.mult_ac(1) transformation_left_frame mult.commute)
-
-lemma [\<phi>reason 1200]:
-  \<open> x \<Ztypecolon> T \<t>\<r>\<a>\<n>\<s>\<f>\<o>\<r>\<m>\<s> y \<Ztypecolon> U \<w>\<i>\<t>\<h> P @action \<A>_structural Act
-\<Longrightarrow> x \<Ztypecolon> \<phi> T \<t>\<r>\<a>\<n>\<s>\<f>\<o>\<r>\<m>\<s> y \<Ztypecolon> \<phi> U \<w>\<i>\<t>\<h> P @action \<A>_structural Act \<close>
-  unfolding Action_Tag_def using \<phi>_cast .
-
-lemma [\<phi>reason 1200]:
-  \<open> x \<Ztypecolon> T \<t>\<r>\<a>\<n>\<s>\<f>\<o>\<r>\<m>\<s> y \<Ztypecolon> U \<s>\<u>\<b>\<j> y. r y \<w>\<i>\<t>\<h> P @action to Target
-\<Longrightarrow> x \<Ztypecolon> \<phi> T \<t>\<r>\<a>\<n>\<s>\<f>\<o>\<r>\<m>\<s> y \<Ztypecolon> \<phi> U \<s>\<u>\<b>\<j> y. r y \<w>\<i>\<t>\<h> P @action to Target \<close>
-  unfolding Action_Tag_def Transformation_def
+(*to depreciate the above!*)
+
+
+lemma "__Return_rule__":
+  \<open> \<p>\<r>\<o>\<c> Return v \<lbrace> X v \<longmapsto> X \<rbrace> \<close>
+  unfolding \<phi>Procedure_def det_lift_def Return_def
+  by clarsimp
+
+lemma semantic_return_\<phi>app:
+  \<open> \<p>\<a>\<r>\<a>\<m> (v \<Turnstile> (y \<Ztypecolon> T))
+\<Longrightarrow> \<p>\<r>\<e>\<m>\<i>\<s>\<e> v \<Turnstile> (y \<Ztypecolon> T)
+\<Longrightarrow> \<p>\<r>\<o>\<c> Return (\<phi>arg v) \<lbrace> X \<longmapsto> \<lambda>u. X\<heavy_comma> y \<Ztypecolon> Val u T \<rbrace> \<close>
+  unfolding Premise_def \<phi>Procedure_def det_lift_def Return_def
+  by (clarsimp simp add: Val.unfold)
+
+lemma semantic_literal_\<phi>app:
+  \<open> \<p>\<a>\<r>\<a>\<m> (v \<Turnstile> (y \<Ztypecolon> T))
+\<Longrightarrow> \<p>\<r>\<e>\<m>\<i>\<s>\<e> v \<Turnstile> (y \<Ztypecolon> T)
+\<Longrightarrow> Void \<t>\<r>\<a>\<n>\<s>\<f>\<o>\<r>\<m>\<s> y \<Ztypecolon> Val (semantic_literal v) T \<close>
+  unfolding Premise_def Transformation_def semantic_literal_def
+  by clarsimp
+
+lemma semantic_local_value_\<phi>app:
+  \<open> \<p>\<a>\<r>\<a>\<m> TY
+\<Longrightarrow> \<phi>SemType (x \<Ztypecolon> T) TY
+\<Longrightarrow> \<p>\<r>\<o>\<c> \<phi>M_assert (\<phi>arg.dest v \<in> Well_Type TY) \<lbrace> x \<Ztypecolon> \<v>\<a>\<l>[v] T \<longmapsto> \<lambda>_. Void \<s>\<u>\<b>\<j> \<phi>arg.dest v \<Turnstile> (x \<Ztypecolon> T) \<rbrace>\<close>
+  unfolding \<phi>M_assert_def Premise_def \<phi>SemType_def subset_iff \<phi>Procedure_def det_lift_def Return_def
+  by (clarsimp simp add: Val.unfold INTERP_SPEC Satisfaction_def Subjection_expn_set)
+
+lemma semantic_local_values_nochk_\<phi>app:
+  \<open> x \<Ztypecolon> \<v>\<a>\<l>\<s>[v] T \<t>\<r>\<a>\<n>\<s>\<f>\<o>\<r>\<m>\<s> Void \<w>\<i>\<t>\<h> \<phi>arg.dest v \<Turnstile> (x \<Ztypecolon> T) \<close>
+  unfolding Transformation_def
   by clarsimp
 
 
-lemma [\<phi>reason 1200]:
-  \<open> Identity_Element\<^sub>I (x \<Ztypecolon> T) P
-\<Longrightarrow> Identity_Element\<^sub>I (x \<Ztypecolon> \<phi> T) P \<close>
-  unfolding Identity_Element\<^sub>I_def Transformation_def apply simp
-  using mk_homo_one by blast
-
-lemma [\<phi>reason 1200 for \<open>If _ (_ \<Ztypecolon> \<phi> _) (_ \<Ztypecolon> \<phi> _) \<t>\<r>\<a>\<n>\<s>\<f>\<o>\<r>\<m>\<s> _ @action br_join\<close>]:
-  \<open> If P (x \<Ztypecolon> T) (y \<Ztypecolon> U) \<t>\<r>\<a>\<n>\<s>\<f>\<o>\<r>\<m>\<s> (z \<Ztypecolon> Z) @action br_join
-\<Longrightarrow> If P (x \<Ztypecolon> \<phi> T) (y \<Ztypecolon> \<phi> U) \<t>\<r>\<a>\<n>\<s>\<f>\<o>\<r>\<m>\<s> (z \<Ztypecolon> \<phi> Z) @action br_join\<close>
-  unfolding Action_Tag_def by (cases P; simp add: \<phi>_cast)
-
-paragraph \<open>Conversion\<close>
-
-lemma [simp]:
-  \<open>(\<phi> (ExTyp T)) = (\<exists>\<phi> c. \<phi> (T c))\<close>
-  by (rule \<phi>Type_eqI; simp; blast)
-
-(*lemma [simp]: TODO!!!!
-  \<open>(\<phi> (T \<phi>\<s>\<u>\<b>\<j> P)) = (\<phi> T \<phi>\<s>\<u>\<b>\<j> P)\<close>
-  by (rule \<phi>Type_eqI; clarsimp simp add: \<phi>expns; blast)*)
-
-lemma \<phi>_simp_cong[folded atomize_eq]:
-  \<open> (x \<Ztypecolon> T) = (x' \<Ztypecolon> T')
-\<Longrightarrow> (x \<Ztypecolon> \<phi> T) = (x' \<Ztypecolon> \<phi> T')\<close>
-  unfolding BI_eq_iff by simp
-
-simproc_setup \<phi>\<phi>_simp_cong ("x \<Ztypecolon> \<phi> T") = \<open>
-  K (fn ctxt => Phi_SimpProc.cong @{thm \<phi>_simp_cong} ctxt)
-\<close>
-
-paragraph \<open>Synthesis for moving\<close>
-
-lemma [\<phi>reason 1200 for
-  \<open>Synthesis_Parse (\<phi> ?T) (?Y::?'ret \<Rightarrow> assn)\<close>
-]:
-  \<open>Synthesis_Parse (\<phi> T) (\<lambda>_. x \<Ztypecolon> \<phi> T :: assn)\<close>
-  unfolding Synthesis_Parse_def ..
-
-(* lemma [\<phi>reason for \<open>\<p>\<r>\<o>\<c> ?f \<lbrace> ?S1 \<longmapsto> \<lambda>ret. ?S2\<heavy_comma>  \<blangle> ?x \<Ztypecolon> \<phi> ?T \<brangle> \<rbrace> \<t>\<h>\<r>\<o>\<w>\<s> ?E\<close>]:
-  \<open> SUBGOAL G G'
-\<Longrightarrow> S1 \<t>\<r>\<a>\<n>\<s>\<f>\<o>\<r>\<m>\<s> S2\<heavy_comma> \<blangle> x \<Ztypecolon> \<phi> T \<brangle>
-\<Longrightarrow> SOLVE_SUBGOAL G'
-\<Longrightarrow> \<p>\<r>\<o>\<c> Return \<phi>V_none \<lbrace> S1 \<longmapsto> \<lambda>_. S2\<heavy_comma> \<blangle> x \<Ztypecolon> \<phi> T \<brangle> \<rbrace>\<close>
-  unfolding FOCUS_TAG_def Synthesis_def Action_Tag_def
-  using \<phi>__Return_rule__ view_shift_by_implication by blast *)
-
-end
-
-
-subsubsection \<open>Permission Fiction\<close>
-
-locale permission_fiction =
-   R: resource Res
-+  share: share_orthogonal_homo \<psi> UNIV
-+  fiction_kind FIC.DOMAIN INTERPRET Fic
-      \<open>R.basic_fiction \<Zcomp>\<^sub>\<I> (\<F>_functional \<psi> UNIV)\<close>
-for Res :: "'T::sep_algebra resource_entry"
-and \<psi> :: \<open>'T \<Rightarrow> 'U::{share_sep_disj,share_semimodule,sep_algebra}\<close>
-and Fic :: "'U fiction_entry"
-+ assumes \<psi>_kernel_is_1[simp]: \<open>kernel_is_1 \<psi> UNIV\<close>
-begin
-
-sublocale basic_fiction Res \<open>\<F>_functional \<psi> UNIV\<close> ..
-
-thm interp_split
-
-lemma sep_disj_fiction:
-  \<open> r \<in> FIC.SPACE
-\<Longrightarrow> \<s>\<t>\<a>\<t>\<e> s \<i>\<s> INTERP r * { R.mk x }
-\<Longrightarrow> r ## mk (\<psi> x)\<close>
-  unfolding \<phi>Res_Sat_def \<phi>Res_Spec_def set_eq_iff
-  apply (clarsimp simp add: R.basic_fiction_def set_mult_expn
-            \<phi>Res_Spec_def R.\<r>_valid_split'
-            R.inj.sep_orthogonal interp_split[where f=r, simplified]
-            sep_disj_get_name_eq[symmetric]
-            simp del: sep_disj_get_name_eq)
-  using sep_disj_multD2 by force
-
-lemma expand_subj:
-  \<open> r \<in> FIC.SPACE
-\<Longrightarrow> \<phi>Res_Spec (INTERP (r * mk (\<psi> x)) \<s>\<u>\<b>\<j> r ## mk (\<psi> x))
-  = \<phi>Res_Spec (INTERP r * { R.mk x })\<close>
-  unfolding \<phi>Res_Spec_def set_eq_iff
-  apply (clarify, rule)
-  apply (clarsimp simp add: R.basic_fiction_def set_mult_expn Subjection_expn_set
-            share.sep_orthogonal \<phi>Res_Spec_def R.\<r>_valid_split'
-            R.inj.sep_orthogonal interp_split[simplified] prj.homo_mult)
-  subgoal for res_r a r'
-    apply (rule exI[where x=\<open>res_r * R.mk a\<close>]; rule)
-    apply (metis R.inj.homo_mult R.sep_disj_mk fun_1upd_homo_right1 sep_mult_assoc')
-    by (metis R.mk_homo_mult R.sep_disj_mk sep_disj_multD1 sep_disj_multI1)
-
-  apply (clarsimp simp add: R.basic_fiction_def set_mult_expn Subjection_expn_set \<phi>Res_Spec_def R.\<r>_valid_split'
-        R.inj.sep_orthogonal interp_split[simplified] sep_mult_assoc prj.homo_mult)
-  subgoal premises prems for res_r a y proof -
-    have t1[simp]: \<open>y ## x\<close>
-      using prems(5) prems(7) sep_disj_multD2 by force
-
-    show ?thesis
-      apply rule
-      apply (rule exI[where x=\<open>a\<close>], rule exI[where x=\<open>R.mk (y * x)\<close>])
-      apply (metis R.inj.homo_mult fun_1upd_homo prems(5) prems(6) prems(7) sep_disj_multI2 share.homo_mult t1)
-      by (metis prems(1) prems(8) sep_disj_get_name_eq share.sep_disj_homo_semi t1)
-
-  qed .
-
-lemma expand:
-  \<open> r \<in> FIC.SPACE
-\<Longrightarrow> r ## mk (\<psi> x)
-\<Longrightarrow> \<phi>Res_Spec (INTERP (r * mk (\<psi> x))) =
-    \<phi>Res_Spec (INTERP r * {R.mk x})\<close>
-  subgoal premises prems
-    using expand_subj[where r=r and x=x, simplified prems(2) Subjection_True, OF prems(1)] . .
-
-(*lemma expand_conj:
-  \<open> r \<in> FIC.SPACE
-\<Longrightarrow> (\<s>\<t>\<a>\<t>\<e> s \<i>\<s> \<I> INTERP (r * mk (share_orthogonal_homo x))) \<and> r ## mk (share_orthogonal_homo x)
-\<longleftrightarrow> (\<s>\<t>\<a>\<t>\<e> s \<i>\<s> \<I> INTERP r * { R.mk x })\<close>
-  unfolding \<phi>Res_Sat_def
-  subgoal premises prems
-    using expand_subj[where r=r and x=x, OF prems(1)]
-      by (simp add: \<phi>expns) . *)
-
-
-lemma partial_implies_raw:
-  \<open> r \<in> FIC.SPACE
-\<Longrightarrow> 0 < n
-\<Longrightarrow> r ## mk (share n (\<psi> x))
-\<Longrightarrow> \<s>\<t>\<a>\<t>\<e> res \<i>\<s> INTERP (r * mk (share n (\<psi> x)))
-\<Longrightarrow> x \<preceq>\<^sub>S\<^sub>L R.get res\<close>
-  unfolding \<phi>Res_Spec_def \<phi>Res_Sat_def
-  apply (clarsimp simp add: R.basic_fiction_def set_mult_expn Subjection_expn_set
-            \<phi>Res_Spec_def R.\<r>_valid_split' R.inj.sep_orthogonal
-            R.prj.homo_mult interp_split[simplified] prj.homo_mult)
-  apply (cases \<open>n \<le> 1\<close>)
-  apply (metis UNIV_I join_sub_def join_sub_ext_left sep_space_entry.sep_disj_get_name sep_space_entry_axioms share.join_sub_share_join_sub_whole)
-  subgoal premises prems for u y a proof -
-    have t0: \<open>1 / n * n = 1\<close>
-      by (metis nonzero_eq_divide_eq order_less_irrefl prems(2))
-    have t1: \<open>1 / n \<le> 1 \<and> 0 < 1 / n\<close>
-      using prems(13) by force
-    have t2: \<open>share (1/n) (share n (\<psi> x)) \<preceq>\<^sub>S\<^sub>L share n (\<psi> x)\<close>
-      by (simp add: order_less_imp_le prems(2) share.\<psi>_mul_carrier share_sub t1)
-    then have t3: \<open>\<psi> x \<preceq>\<^sub>S\<^sub>L share n (\<psi> x)\<close>
-      using share_share_assoc0
-      by (metis prems(2) share_left_one t0 t1
-    then show ?thesis
-      by (metis UNIV_I join_sub_ext_let prems(10) prems(3) prems(8) sep_disj_get_name share.homo_join_sub)
-  qed .
-
-paragraph \<open>Reasoning Rules\<close>
-
-(*
-declare NToA_by_structural_extraction
-    [\<phi>reason 1210 if \<open>PLPR_Env.boolean_flag \<^const_name>\<open>ToA_flag_deep\<close> true o fst\<close>]
-declare NToA_by_structural_extraction__reverse_transformation
-    [\<phi>reason 1213 if \<open>PLPR_Env.boolean_flag \<^const_name>\<open>ToA_flag_deep\<close> true o fst\<close>]
-*)
-end
-
-
-
-
-
-subsubsection \<open>Itself Fiction\<close>
-
-locale identity_fiction =
-   R: resource Res
-+  fiction_kind FIC.DOMAIN INTERPRET Fic \<open>R.basic_fiction \<Zcomp>\<^sub>\<I> \<F>_it\<close>
-for Res :: "'T::sep_algebra resource_entry"
-and Fic :: "'T fiction_entry"
-begin
-
-sublocale basic_fiction where I = \<open>\<F>_it\<close> ..
-
-lemma sep_disj_fiction:
-  \<open> r \<in> FIC.SPACE
-\<Longrightarrow> \<s>\<t>\<a>\<t>\<e> s \<i>\<s> INTERP r * { R.mk x }
-\<Longrightarrow> r ## mk x\<close>
-  unfolding \<phi>Res_Sat_def \<phi>Res_Spec_def set_eq_iff
-  apply (clarsimp simp add: R.basic_fiction_def set_mult_expn Subjection_expn_set
-            \<phi>Res_Spec_def R.\<r>_valid_split'
-            R.inj.sep_orthogonal interp_split[simplified]
-            sep_disj_get_name_eq[symmetric]
-            simp del: sep_disj_get_name_eq)
-  using sep_disj_multD2 by force
-
-lemma expand_subj:
-  \<open> r \<in> FIC.SPACE
-\<Longrightarrow> (\<phi>Res_Spec (INTERP (r * mk x) \<s>\<u>\<b>\<j> r ## mk x)) = \<phi>Res_Spec (INTERP r * {R.mk x}) \<close>
-  unfolding \<phi>Res_Spec_def set_eq_iff
-  apply (clarify; rule; clarsimp simp add: set_mult_expn Subjection_expn_set R.basic_fiction_def interp_split[simplified] prj.homo_mult)
-  apply (simp add: R.mk_homo_mult)
-  apply (metis (no_types, lifting) R.sep_disj_mk sep_disj_get_name sep_disj_multD1 sep_disj_multI1 sep_mult_assoc')
-  apply (simp add: R.mk_homo_mult[symmetric] sep_mult_assoc)
-  by (metis R.mk_homo_mult R.sep_disj_mk sep_disj_get_name_eq sep_disj_multD2 sep_disj_multI2)
-
-lemma expand:
-  \<open> r \<in> FIC.SPACE
-\<Longrightarrow> r ## mk x
-\<Longrightarrow> \<phi>Res_Spec (INTERP (r * mk x)) = \<phi>Res_Spec (INTERP r * {R.mk x})\<close>
-  subgoal premises prems
-    using expand_subj[where r=r and x=x, simplified prems(2) Subjection_True, OF prems(1)] . .
-
-(*
-declare NToA_by_structural_extraction
-   [\<phi>reason 1210 if \<open>PLPR_Env.boolean_flag \<^const_name>\<open>ToA_flag_deep\<close> true o fst\<close>]
-declare NToA_by_structural_extraction__reverse_transformation
-   [\<phi>reason 1213 if \<open>PLPR_Env.boolean_flag \<^const_name>\<open>ToA_flag_deep\<close> true o fst\<close>]
-*)
-end
-
-
-subsection \<open>Discrete Monolithic Resource\<close>
-  \<comment> \<open>The resource non-sepable and having type shape \<^typ>\<open>'a::discrete_semigroup option\<close>\<close>
-
-(* locale discrete_mono_resource =
-  resource Res
-for Res :: "'T discrete option resource_entry"
-begin
-
-definition fiction_agree
-  where \<open>fiction_agree = basic_fiction \<Zcomp>\<^sub>\<I> \<F>_optionwise \<F>_agree\<close>
-
-end
-
-
-subsubsection \<open>Interp Agreement\<close>
-
-(*TODO: ('k \<Rightarrow> 'v) discrete option ----> ('k \<Rightarrow> 'v share option)
-  total to that
-  none to none
- *)
-
-locale agreement_fiction_for_discrete_mono_resource =
-   R: discrete_mono_resource Res
-+  fiction_kind FIC.DOMAIN INTERPRET Fic \<open>R.fiction_agree\<close>
-for Res :: "'T discrete option resource_entry"
-and Fic :: "'T discrete agree option fiction_entry"
-begin
-
-sublocale basic_fiction Res \<open>\<F>_optionwise \<F>_agree\<close> Fic
-  by (standard; simp add: R.fiction_agree_def raw_domain)
-
-lemma partial_implies:
-  \<open> r \<in> FIC.SPACE
-\<Longrightarrow> r ## mk (Some (agree (discrete x)))
-\<Longrightarrow> \<s>\<t>\<a>\<t>\<e> res \<i>\<s> \<I> INTERP (r * mk (Some (agree (discrete x))))
-\<Longrightarrow> R.get res = Some (discrete x)\<close>
-  unfolding \<phi>Res_Spec_def \<phi>Res_Sat_def
-  apply (clarsimp simp add: interp_split'
-     R.fiction_agree_def R.basic_fiction_\<I> interp_comp_\<I> \<phi>expns R.\<r>_valid_split'
-     R.inject_wand_homo R.prj.homo_mult \<F>_optionwise_\<I> image_iff Bex_def
-     \<F>_agree_def prj.homo_mult)
-  apply (cases \<open>get r\<close>; simp)
-  subgoal for u y a aa
-    apply (cases aa; simp)
-    subgoal premises prems for xa proof -
-      have \<open>get r ## Some (agree (discrete x))\<close>
-        by (metis prems(2) sep_disj_get_name)
-      from this [unfolded \<open>get r = _\<close>, simplified]
-      show ?thesis .
-    qed . .
-
-lemma double:
-  \<open>{mk x |x. P x} \<t>\<r>\<a>\<n>\<s>\<f>\<o>\<r>\<m>\<s> {mk x |x. P x} * {mk x |x. P x}\<close>
+lemma semantic_local_value_nochk_\<phi>app:
+  \<open> x \<Ztypecolon> \<v>\<a>\<l>[v] T \<t>\<r>\<a>\<n>\<s>\<f>\<o>\<r>\<m>\<s> 1 \<w>\<i>\<t>\<h> \<phi>arg.dest v \<Turnstile> (x \<Ztypecolon> T) \<close>
   unfolding Transformation_def
-  apply (clarsimp simp add: \<phi>expns mk_homo_mult[symmetric])
-  subgoal for x'
-    apply (rule exI[where x=\<open>mk x'\<close>], rule exI[where x=\<open>mk x'\<close>])
-    by (cases x'; simp add: mk_homo_mult[symmetric]) .
-
-lemma contract:
-  \<open>{mk x |x. P x} * {mk x |x. P x} \<t>\<r>\<a>\<n>\<s>\<f>\<o>\<r>\<m>\<s> {mk x |x. P x} \<close>
-  unfolding Transformation_def
-  apply (clarsimp simp add: \<phi>expns)
-  subgoal for x y by (cases x; cases y; simp add: mk_homo_mult[symmetric]) .
-
-paragraph \<open>\<phi>-Type\<close>
-
-abbreviation \<open>\<phi>_ag T \<equiv> \<phi> (Agreement (Discrete T))\<close>
-
-(*declare NToA_by_structural_extraction
-    [\<phi>reason 1210 if \<open>PLPR_Env.boolean_flag \<^const_name>\<open>ToA_flag_deep\<close> true o fst\<close>]
-declare NToA_by_structural_extraction__reverse_transformation
-    [\<phi>reason 1213 if \<open>PLPR_Env.boolean_flag \<^const_name>\<open>ToA_flag_deep\<close> true o fst\<close>]
-*)
-
-lemma \<phi>_double_\<phi>app:
-  \<open>x \<Ztypecolon> \<phi>_ag T \<t>\<r>\<a>\<n>\<s>\<f>\<o>\<r>\<m>\<s> x \<Ztypecolon> \<phi>_ag T \<heavy_comma> x \<Ztypecolon> \<phi>_ag T\<close>
-proof -
-  have \<open>\<exists>P. (x \<Ztypecolon> \<phi>_ag T) = {mk x |x. P x}\<close>
-    unfolding set_eq_iff apply (simp add: \<phi>expns)
-    apply (rule exI[where x=\<open>\<lambda>y. \<exists>v. y = Some (agree (discrete v)) \<and> v \<in> (x \<Ztypecolon> T)\<close>])
-    by blast
-  then obtain P where [simp]: \<open>(x \<Ztypecolon> \<phi>_ag T) = {mk x |x. P x}\<close> by blast
-  show ?thesis by (simp add: double)
-qed
-
-lemma \<phi>_contract_\<phi>app:
-  \<open>x \<Ztypecolon> \<phi>_ag T \<heavy_comma> x \<Ztypecolon> \<phi>_ag T \<t>\<r>\<a>\<n>\<s>\<f>\<o>\<r>\<m>\<s> x \<Ztypecolon> \<phi>_ag T\<close>
-proof -
-  have \<open>\<exists>P. (x \<Ztypecolon> \<phi>_ag T) = {mk x |x. P x}\<close>
-    unfolding set_eq_iff apply (simp add: \<phi>expns)
-    apply (rule exI[where x=\<open>\<lambda>y. \<exists>v. y = Some (agree (discrete v)) \<and> v \<in> (x \<Ztypecolon> T)\<close>])
-    by blast
-  then obtain P where [simp]: \<open>(x \<Ztypecolon> \<phi>_ag T) = {mk x |x. P x}\<close> by blast
-  show ?thesis by (simp add: contract)
-qed
-
-end
-
-*)
-
-subsection \<open>Resources based on Mapping\<close>
-
-locale mapping_resource =
-  resource Res
-for Res :: "('key \<Rightarrow> 'val::sep_algebra) resource_entry"
-begin
-
-lemma "__allocation_rule__":
-  \<open> (\<forall>m. m \<in>\<^sub>S\<^sub>H domain \<longrightarrow> m(k := u) \<in>\<^sub>S\<^sub>H domain)
-\<Longrightarrow> k \<notin> dom1 (get res)
-\<Longrightarrow> \<s>\<t>\<a>\<t>\<e> res \<i>\<s> R
-\<Longrightarrow> \<s>\<t>\<a>\<t>\<e> updt (\<lambda>f. f(k := u)) res \<i>\<s> R * {mk (1(k := u))}\<close>
-  unfolding \<phi>Res_Sat_def \<phi>Res_Spec_def
-  apply (clarsimp simp add: \<r>_valid_split' times_set_def inj.sep_orthogonal
-          prj.homo_mult times_fun_upd)
-  subgoal premises prems for m proof -
-    {
-      assume A: \<open>k \<notin> dom1 m\<close>
-      have t2: \<open>m ## 1(k := u)\<close>
-        using A dom1_def sep_disj_fun_def by fastforce
-      have t3: \<open>res(name := inject m) = res\<close>
-        by (simp add: fun_upd_idem prems(5))
-      have t1: \<open>res(name := inject (m(k := u))) = res * mk (1(k := u)) \<and> res ## mk (1(k := u))\<close>
-        thm fun_split_1_not_dom1[where f=m]
-        apply (subst fun_split_1_not_dom1[where k=k]) using A apply this
-        apply (simp add: t2 inj.homo_mult split)
-        by (metis fun_1upd_homo_right1 fun_sep_disj_1_fupdt(1) inj.sep_disj_homo_semi t2 t3)
-    }
-    then show ?thesis
-      using prems(2) prems(4) by blast
-  qed .
-
-end
-
-subsection \<open>One Level Parital Mapping\<close>
-
-subsubsection \<open>Locale for Resource\<close>
-
-locale partial_map_resource =
-  mapping_resource Res
-for Res :: "('key \<Rightarrow> 'val::discrete_semigroup option) resource_entry"
-begin
-
-lemma "__updt_rule__":
-  \<open> (\<forall>m. m \<in>\<^sub>S\<^sub>H domain \<longrightarrow> P m \<longrightarrow> m(k := u) \<in>\<^sub>S\<^sub>H domain)
-\<Longrightarrow> P (get res)
-\<Longrightarrow> \<s>\<t>\<a>\<t>\<e> res \<i>\<s> R * {mk (1(k \<mapsto> any))}
-\<Longrightarrow> \<s>\<t>\<a>\<t>\<e> updt (\<lambda>f. f(k := u)) res \<i>\<s> R * {mk (1(k := u))}\<close>
-  unfolding \<phi>Res_Sat_def \<phi>Res_Spec_def
-  apply (clarsimp simp add: \<r>_valid_split' times_set_def inj.sep_orthogonal
-          prj.homo_mult times_fun_upd )
-  apply (clarsimp simp add: sep_disj_partial_map_upd
-          discrete_semigroup_sepdisj_fun mk_homo_mult)
-  subgoal premises prems for x aa proof -
-    have t1: \<open>clean x * mk aa = x\<close>
-      by (metis fun_split_1 prems(7))
-    have t2: \<open>clean x ## (mk aa * mk (1(k := u)))\<close>
-      by (simp add: fun_1upd_homo)
-    show ?thesis
-      by (metis (no_types, opaque_lifting) fun_1upd_homo_right1 fun_sep_disj_1_fupdt(1) inj.sep_disj_homo_semi mult_1_class.mult_1_left discrete_semigroup_sepdisj_fun prems(5) prems(8) t1)
-  qed .
-
-lemma "__dispose_rule__":
-  \<open> (\<forall>m. m \<in>\<^sub>S\<^sub>H domain \<longrightarrow> P m \<longrightarrow> m(k := None) \<in>\<^sub>S\<^sub>H domain)
-\<Longrightarrow> P (get res)
-\<Longrightarrow> \<s>\<t>\<a>\<t>\<e> res \<i>\<s> R * {mk (1(k \<mapsto> any))}
-\<Longrightarrow> \<s>\<t>\<a>\<t>\<e> updt (\<lambda>f. f(k := None)) res \<i>\<s> R\<close>
-  using "__updt_rule__"[where u=None, simplified, simplified,
-            simplified, simplified one_set_def[symmetric], simplified] .
-
-(*depreciate*)
-abbreviation share_orthogonal_homo :: \<open>('key \<Rightarrow> 'val option) \<Rightarrow> ('key \<Rightarrow> 'val share option)\<close>
-  where \<open>share_orthogonal_homo \<equiv> (o) to_share\<close>
-(*depreciate*)
-abbreviation \<open>share_fiction \<equiv> basic_fiction \<Zcomp>\<^sub>\<I> \<F>_functional share_orthogonal_homo UNIV\<close>
-
-(* lemma share_fiction_expn_full:
-  \<open>\<phi>Res_Spec (R * \<I> share_fiction (R2 * Fine (1(k \<mapsto> 1 \<odiv> v))))
- = \<phi>Res_Spec (R * \<I> share_fiction R2 * { mk (Fine (1(k \<mapsto> v)))})\<close>
-  unfolding set_eq_iff
-  apply (clarify, rule;
-         clarsimp simp add: share_fiction_def basic_fine_fiction_\<I> \<phi>expns fiction_to_share_\<I>
-            mult_strip_fine_011 \<phi>Res_Spec_def \<r>_valid_split' inject_wand_homo)
-  subgoal premises prems for res_r y a r
-    apply (insert \<open>a * _ = _\<close>[unfolded to_share_wand_homo[where b=\<open>1(k \<mapsto> v)\<close>, simplified, OF \<open>a ## _\<close>]])
-    apply (clarsimp simp add: times_fine'[symmetric] mk_homo_mult mult.assoc[symmetric])
-    using prems(3) by blast
-  subgoal premises prems for res_r a r proof -
-    have t1[simp]: \<open>a ## 1(k \<mapsto> v)\<close>
-      by (metis prems(6) prems(7) sep_disj_commuteI sep_disj_multD1 sep_mult_commute)
-    show ?thesis
-    apply (clarsimp simp add: mult.assoc mk_homo_mult[symmetric] times_fine')
-      apply (rule exI[where x=res_r], rule exI[where x="mk (Fine (a * 1(k \<mapsto> v)))"], simp add: prems)
-      by (metis (no_types, lifting) map_option_o_map_upd t1 to_share_funcomp_1 to_share_funcomp_sep_disj_I to_share_wand_homo)
-  qed .
-
-
-lemma share_fiction_partially_implies:
-  \<open> res \<in> \<phi>Res_Spec (R * \<I> share_fiction (R2 * Fine (1(k \<mapsto> n \<odiv> v))))
-\<Longrightarrow> \<exists>objs. get res = Fine objs \<and> objs k = Some v\<close>
-  apply (clarsimp simp add: share_fiction_def basic_fine_fiction_\<I> \<phi>expns fiction_to_share_\<I>
-            mult_strip_fine_011 \<phi>Res_Spec_def \<r>_valid_split' inject_wand_homo
-            proj_homo_mult)
-  subgoal premises prems for res_r y a r proof -
-    from \<open>a * _ = _\<close>[THEN fun_cong[where x=k], simplified times_fun, simplified]
-    have t1: \<open>y k = Some v\<close>
-      using prems(6) prems(7) strip_share_fun_mult by force
-    then show ?thesis apply (simp add: t1 times_fun)
-      using prems(9) sep_disj_partial_map_some_none t1 by fastforce
-  qed .
-
-lemma
-  assumes A: \<open> res \<in> \<phi>Res_Spec (R * \<I> share_fiction (R2 * Fine (1(k \<mapsto> n \<odiv> v))))\<close>
-  shows share_fiction_partially_implies'[simp]: \<open>!!( get res) k = Some v\<close>
-proof -
-  from A[THEN share_fiction_partially_implies]
-  show ?thesis by fastforce
-qed
-*)
-lemma raw_unit_assertion_implies[simp]:
-  \<open> \<s>\<t>\<a>\<t>\<e> res \<i>\<s> R * { mk (1(k \<mapsto> v))}
-\<Longrightarrow> get res k = Some v\<close>
-  unfolding \<phi>Res_Sat_def \<phi>Res_Spec_def
-  apply (clarsimp simp add: times_set_def \<r>_valid_split' inj.sep_orthogonal
-      prj.homo_mult sep_disj_fun_def times_fun)
-  by (metis mult_1_class.mult_1_left one_option_def option.simps(3))
-
-
-end
-
-subsubsection \<open>Itself Fiction\<close>
-
-locale identity_fiction_for_partial_mapping_resource =
-   R: partial_map_resource Res
-+  fiction_kind FIC.DOMAIN INTERPRET Fic \<open>R.basic_fiction \<Zcomp>\<^sub>\<I> \<F>_it\<close>
-for Res :: "('key \<Rightarrow> 'val::discrete_semigroup option) resource_entry"
-and Fic :: "('key \<Rightarrow> 'val option) fiction_entry"
-begin
-
-sublocale identity_fiction Res Fic ..
-
-end
-
-
-subsubsection \<open>Permission Fiction\<close>
-
-locale share_fiction_for_partial_mapping_resource =
-   R: partial_map_resource Res
-+  fiction_kind FIC.DOMAIN INTERPRET Fic \<open>R.share_fiction\<close>
-for Res :: "('key \<Rightarrow> 'val::discrete_semigroup option) resource_entry"
-and Fic :: "('key \<Rightarrow> 'val share option) fiction_entry"
-begin
-
-sublocale permission_fiction Res \<open>R.share_orthogonal_homo\<close>
-  by (standard; simp add: pointwise_set_UNIV kernel_is_1_def)
-
-lemma expand:
-  \<open> r \<in> FIC.SPACE
-\<Longrightarrow> r ## mk (R.share_orthogonal_homo x)
-\<Longrightarrow> \<phi>Res_Spec (INTERP (r * mk (R.share_orthogonal_homo x))) =
-    \<phi>Res_Spec (INTERP r * {R.mk x} )\<close>
-  subgoal premises prems
-    using expand_subj[where r=r and x=x, simplified prems(2) Subjection_True, OF prems(1)] . .
-
-lemma partial_implies:
-  \<open> r \<in> FIC.SPACE
-\<Longrightarrow> 0 < n
-\<Longrightarrow> r ## mk (1(k \<mapsto> Share n v))
-\<Longrightarrow> \<s>\<t>\<a>\<t>\<e> res \<i>\<s> INTERP (r * mk (1(k \<mapsto> Share n v)))
-\<Longrightarrow> R.get res k = Some v\<close>
-  using partial_implies_raw[where x=\<open>1(k \<mapsto> v)\<close> and n=n, simplified]
-    discrete_partial_map_subsumption
-  by (smt (verit, ccfv_threshold) fun_split_1 fun_upd_same join_sub_def one_option_def sep_disj_fun_def sep_disj_option_discrete(1) times_fupdt_1_apply_sep)
-
-lemma partial_implies'[simp]:
-  assumes FS: \<open>r \<in> FIC.SPACE\<close>
-    and N: \<open>0 < n\<close>
-    and S: \<open>r ## mk (1(k \<mapsto> Share n v))\<close>
-    and A: \<open>\<s>\<t>\<a>\<t>\<e> res \<i>\<s> INTERP (r * mk (1(k \<mapsto> Share n v)))\<close>
-  shows \<open>R.get res k = Some v\<close>
-proof -
-  from partial_implies[OF FS, OF N, OF S, OF A]
-  show ?thesis by fastforce
-qed
-
-(* lemma VS_merge_ownership_identity:
-  \<open> na + nb \<le> 1
-\<Longrightarrow> x \<Ztypecolon> \<phi> (share.\<phi> na Itself) \<heavy_comma> x \<Ztypecolon> \<phi> (share.\<phi> nb Itself) \<t>\<r>\<a>\<n>\<s>\<f>\<o>\<r>\<m>\<s> x \<Ztypecolon> \<phi> (share.\<phi> (na + nb) Itself)\<close>
-  by (rule VS_merge_ownership; simp add: \<phi>expns)
-
-lemma VS_split_ownership_identity:
-  \<open> \<p>\<r>\<e>\<m>\<i>\<s>\<e> (0 < n \<longrightarrow> na + nb = n \<and> 0 < na \<and> 0 < nb)
-\<Longrightarrow> x \<Ztypecolon> \<phi> (share.\<phi> n Itself) \<t>\<r>\<a>\<n>\<s>\<f>\<o>\<r>\<m>\<s> x \<Ztypecolon> \<phi> (share.\<phi> na Itself) \<heavy_comma> x \<Ztypecolon> \<phi> (share.\<phi> nb Itself)\<close>
-  by (rule VS_split_ownership; simp add: \<phi>expns sep_disj_fun_def share_fun_def; clarify)
-  (* subgoal premises prems for a
-    by (insert \<open>\<forall>_. _\<close>[THEN spec[where x=a]], cases \<open>x a\<close>; simp add: share_All prems) . *)
-
-
-lemma VS_divide_ownership:
-  \<open>FIX x \<Ztypecolon> \<phi> (share.\<phi> n Itself) \<t>\<r>\<a>\<n>\<s>\<f>\<o>\<r>\<m>\<s> x \<Ztypecolon> \<phi> (share.\<phi> (1/2*n) Itself) \<heavy_comma> x \<Ztypecolon> \<phi> (share.\<phi> (1/2*n) Itself)\<close>
-  unfolding Fix_def
-  by (rule VS_split_ownership_identity; simp add: Premise_def)
-*)
-end
-
-locale share_fiction_for_partial_mapping_resource_discrete =
-  share_fiction_for_partial_mapping_resource Res Fic
-for Res :: "('key \<Rightarrow> 'val discrete option) resource_entry"
-and Fic :: "('key \<Rightarrow> 'val discrete share option) fiction_entry"
-begin
-
-lemma \<phi>discrete_normalize:
-  \<open>(x \<Ztypecolon> \<phi> (share.\<phi> (\<phi>MapAt addr (\<phi>Some (Discrete Itself)))))
- = (discrete x \<Ztypecolon> \<phi> (share.\<phi> (\<phi>MapAt addr (\<phi>Some Itself))))\<close>
-  unfolding set_eq_iff by (simp add: \<phi>expns)
-
-end
-
-
-
-subsection \<open>Two Level Parital Mapping\<close>
-
-definition \<open>map_fun_at g k f = (\<lambda>x. if x = k then g (f x) else f x)\<close>
-
-lemma map_fun_at_1[simp]: \<open>map_fun_at g k 1 = 1(k := g 1)\<close>
-  unfolding map_fun_at_def fun_eq_iff by simp
-
-lemma map_fun_at_const[simp]:
-  \<open>map_fun_at (\<lambda>_. u) k f = f(k := u)\<close>
-  unfolding map_fun_at_def fun_eq_iff by simp
-
-
-subsubsection \<open>Locale of Resource\<close>
-
-locale partial_map_resource2 =
-  mapping_resource Res
-for Res :: "('key \<Rightarrow> 'key2 \<Rightarrow> 'val::discrete_semigroup option) resource_entry"
-begin
-
-lemma "__updt_rule__":
-  \<open> (\<forall>m. m \<in>\<^sub>S\<^sub>H domain \<longrightarrow> P m \<longrightarrow> map_fun_at (map_fun_at (\<lambda>_. u) k2) k m \<in>\<^sub>S\<^sub>H domain)
-\<Longrightarrow> P (get res)
-\<Longrightarrow> \<s>\<t>\<a>\<t>\<e> res \<i>\<s> R * {mk (1(k := 1(k2 \<mapsto> any)))}
-\<Longrightarrow> \<s>\<t>\<a>\<t>\<e> updt (map_fun_at (map_fun_at (\<lambda>_. u) k2) k) res
-      \<i>\<s> R * {mk (1(k := 1(k2 := u)))} \<close>
-  unfolding \<phi>Res_Sat_def \<phi>Res_Spec_def
-  apply (clarsimp simp add: \<r>_valid_split' times_set_def inj.sep_orthogonal
-          prj.homo_mult times_fun_upd)
-  subgoal premises prems for x aa proof -
-    have [simp]: \<open>aa k k2 = None\<close>
-      by (metis fun_upd_same prems(8) sep_disj_fun_def sep_disj_option_discrete(1))
-    then have [simp]:
-        \<open>map_fun_at (map_fun_at (\<lambda>_. u) k2) k (aa * 1(k := 1(k2 \<mapsto> any)))
-            = aa * 1(k := 1(k2 := u))\<close>
-      unfolding map_fun_at_def fun_eq_iff times_fun_def
-      by simp
-    have t1[simp]: \<open>clean x * mk aa = x\<close>
-      by (metis fun_split_1 prems(7))
-    have t2[simp]: \<open>aa ## 1(k := 1(k2 := u))\<close>
-      by (simp add: sep_disj_fun_def)
-    have t3[simp]:
-      \<open>clean x ## (mk aa * mk (1(k := 1(k2 := u))))\<close>
-      by (simp add: fun_1upd_homo)
-    have t4:
-      \<open>x ## mk (1(k := 1(k2 := u)))\<close>
-      by (metis sep_disj_mk sep_disj_multI1 t1 t2 t3)
-
-    show ?thesis
-      apply (simp add: prems mk_homo_mult sep_mult_assoc')
-      using prems(6) t4
-      by (metis prems(5))
-  qed .
-
-
-lemma "__dispose_rule__":
-  \<open> (\<forall>m. m \<in>\<^sub>S\<^sub>H domain \<longrightarrow> P m \<longrightarrow> m(k:=1) \<in>\<^sub>S\<^sub>H domain)
-\<Longrightarrow> dom (get res k) = dom any
-\<Longrightarrow> P (get res)
-\<Longrightarrow> \<s>\<t>\<a>\<t>\<e> res \<i>\<s> R * {mk (1(k := any))}
-\<Longrightarrow> \<s>\<t>\<a>\<t>\<e> updt (\<lambda>f. f(k := 1)) res \<i>\<s> R\<close>
-  unfolding \<phi>Res_Sat_def \<phi>Res_Spec_def
-  apply (clarsimp simp add: \<r>_valid_split' times_set_def inj.sep_orthogonal
-          prj.homo_mult times_fun_upd )
-  subgoal premises prems for x aa proof -
-    have \<open>dom (aa k) = {}\<close>
-    proof -
-      obtain kk :: "('key2 \<Rightarrow> 'val option) \<Rightarrow> 'key2" where
-        f1: "\<forall>f. 1 \<noteq> f (kk f) \<or> dom f = {}"
-        by (metis dom_eq_empty_conv one_option_def)
-      have "aa k ## any"
-        by (metis fun_upd_same prems(9) sep_disj_fun)
-      then have "\<forall>ka. 1 = aa k ka \<or> 1 = any ka"
-        by (metis one_option_def option.exhaust sep_disj_fun_discrete(2))
-      then show ?thesis
-        by (metis domIff f1 mult_1_class.mult_1_right one_option_def prems(2) times_fun)
-    qed
-    then have t1[simp]: \<open>(aa * 1(k := any))(k := 1) = aa\<close>
-      by (smt (verit, del_insts) Diff_iff dom1_upd dom_1 dom_eq_empty_conv fun_split_1_not_dom1 fun_upd_triv fun_upd_upd insertCI)
-    have t2[simp]: \<open>clean x * mk aa = x\<close>
-      by (metis fun_split_1 prems(8))
-    show ?thesis
-      using prems(10) prems(6) t1 by force
-  qed .
-
-abbreviation share_orthogonal_homo :: \<open>('key \<Rightarrow> 'key2 \<Rightarrow> 'val option) \<Rightarrow> ('key \<Rightarrow> 'key2 \<Rightarrow> 'val share option)\<close>
-  where \<open>share_orthogonal_homo \<equiv> (o) ((o) to_share)\<close>
-abbreviation \<open>share_fiction \<equiv> basic_fiction \<Zcomp>\<^sub>\<I> \<F>_functional share_orthogonal_homo UNIV\<close>
-
-(*depreciated!*)
-(*lemma share_fiction_expn_full':
-  \<open>\<phi>Res_Spec (R * \<I> share_fiction (R2 * Fine (1(k := to_share o f))))
- = \<phi>Res_Spec (R * \<I> share_fiction R2 * { mk (Fine (1(k := f)))})\<close>
-  unfolding set_eq_iff
-  apply (clarify, rule;
-         clarsimp simp add: share_fiction_def basic_fine_fiction_\<I> \<phi>expns fiction_to_share_\<I>
-            mult_strip_fine_011 \<phi>Res_Spec_def \<r>_valid_split' inject_wand_homo times_fun)
-  subgoal premises prems for res_r y a r
-    apply (insert \<open>\<forall>x. a x * _ = _\<close>[THEN spec[where x=k], simplified,
-          unfolded to_share_wand_homo[where b=f, simplified,
-                      OF sep_disj_fun[where x=k, OF \<open>a ## _\<close>, simplified]]])
-      apply (clarify)
-      subgoal premises prems2 for a' proof -
-        have t1: \<open>y = y(k := a') * 1(k := f)\<close>
-          unfolding fun_eq_iff times_fun
-          apply simp
-          by (metis fun_upd_apply mult_1_class.mult_1_right prems2(2) times_fun_def)
-        have t2: \<open>y(k := a') ## 1(k := f)\<close>
-          using prems2(3) sep_disj_fun_def by fastforce
-        show ?thesis
-          apply (subst t1)
-          apply (clarsimp simp add: times_fine'[OF t2, symmetric] mk_homo_mult mult.assoc[symmetric])
-          apply (rule exI[where x="res_r * mk (Fine (y(k := a')))"], simp)
-          apply (rule exI[where x=res_r], rule exI[where x="mk (Fine (y(k := a')))"], simp add: prems)
-          by (smt (verit, del_insts) mult_1_class.mult_1_right one_fun prems(4) prems2(1))
-      qed .
-    subgoal premises prems for res_r a fic_r r proof -
-      have t1: \<open>a ## 1(k := f)\<close>
-        by (metis prems(7) prems(8) sep_disj_commuteI sep_disj_multD1 sep_mult_commute)
-      have t2: \<open>fic_r ## 1(k := to_share o f)\<close>
-        unfolding sep_disj_fun_def
-        apply (clarsimp)
-        by (metis comp_apply fun_upd_same prems(4) sep_disj_fun_def t1 to_share_funcomp_sep_disj_I)
-
-      show ?thesis
-        apply (clarsimp simp add: mult.assoc mk_homo_mult[symmetric] times_fine'[OF t1])
-        apply (rule exI[where x=res_r], rule exI[where x="mk (Fine (a * 1(k := f))) "],
-                simp add: prems t2)
-        by (smt (verit, best) fun_split_1 fun_upd_def fun_upd_same map_option_o_map_upd prems(4) sep_disj_fun t1 t2 times_fun to_share_funcomp_1 to_share_wand_homo)
-    qed .
-
-lemma share_fiction_expn_full:
-  \<open>\<phi>Res_Spec (R * \<I> share_fiction (R2 * Fine (1(k := 1(k2 \<mapsto> 1 \<odiv> v)))))
- = \<phi>Res_Spec (R * \<I> share_fiction R2 * { mk (Fine (1(k := 1(k2 \<mapsto> v))))})\<close>
-  using share_fiction_expn_full'[where f=\<open>1(k2 \<mapsto> v)\<close>, simplified] .
-
-(*depreciated!*)
-lemma share_fiction_partially_implies:
-  \<open> res \<in> \<phi>Res_Spec (R * \<I> share_fiction (R2 * Fine (1(k := 1(k2 \<mapsto> n \<odiv> v)))))
-\<Longrightarrow> \<exists>objs. get res = Fine objs \<and> objs k k2 = Some v\<close>
-  apply (clarsimp simp add: share_fiction_def basic_fine_fiction_\<I> \<phi>expns fiction_to_share_\<I>
-            mult_strip_fine_011 \<phi>Res_Spec_def \<r>_valid_split' inject_wand_homo
-            proj_homo_mult)
-  subgoal premises prems for res_r y a r proof -
-    note t1 = \<open>a ## _\<close>[THEN sep_disj_fun[where x=k], simplified,
-                 THEN sep_disj_fun[where x=k2], simplified]
-    from \<open>\<forall>_. (a * _) _ = _\<close>[THEN spec[where x=k], simplified times_fun, simplified,
-          THEN fun_cong[where x=k2],
-          simplified times_fun, simplified]
-    have t2: \<open>y k k2 = Some v\<close>
-      using t1 apply (cases \<open>a k k2\<close>; cases \<open>y k k2\<close>; simp)
-      by (metis sep_disj_share share.collapse share.inject times_share)
-
-    then show ?thesis apply (simp add: t2 times_fun)
-      by (metis mult_1_class.mult_1_left one_option_def prems(9) sep_disj_fun sep_disj_option_discrete(1) t2)
-  qed .
-
-lemma
-  assumes A: \<open> res \<in> \<phi>Res_Spec (R * \<I> share_fiction (R2 * Fine (1(k := 1(k2 \<mapsto> n \<odiv> v)))))\<close>
-  shows share_fiction_partially_implies'[simp]: \<open>!!( get res) k k2 = Some v\<close>
-proof -
-  from A[THEN share_fiction_partially_implies]
-  show ?thesis by fastforce
-qed
-*)
-
-lemma raw_unit_assertion_implies[simp]:
-  \<open> \<s>\<t>\<a>\<t>\<e> res \<i>\<s> R * { mk (1(k := 1(k2 \<mapsto> v)))}
-\<Longrightarrow> get res k k2 = Some v\<close>
-  unfolding \<phi>Res_Sat_def \<phi>Res_Spec_def
-  apply (clarsimp simp add: times_set_def \<r>_valid_split' inj.sep_orthogonal
-      prj.homo_mult sep_disj_fun_def times_fun)
-  by (metis fun_upd_same mult_1_class.mult_1_left one_option_def option.discI)
-
-lemma raw_unit_assertion_implies':
-  \<open> \<s>\<t>\<a>\<t>\<e> res \<i>\<s> R * { mk (1(k := f))}
-\<Longrightarrow> f \<subseteq>\<^sub>m get res k\<close>
-  unfolding \<phi>Res_Sat_def \<phi>Res_Spec_def
-  apply (clarsimp simp add: times_set_def \<r>_valid_split' inj.sep_orthogonal)
-  subgoal premises prems for x a proof -
-    have t1[simp]: \<open>inject a ## inject (1(k := f))\<close>
-      using prems(6) by fastforce
-    show ?thesis apply (clarsimp simp add: prj.homo_mult[OF t1] sep_disj_fun_def times_fun map_le_def)
-      by (metis (mono_tags, lifting) fun_sep_disj_1_fupdt(1) fun_upd_triv mult_1_class.mult_1_left one_option_def prems(6) sep_disj_fun_discrete(2))
-  qed .
-
-lemma raw_unit_assertion_implies''[simp]:
-  \<open> \<s>\<t>\<a>\<t>\<e> res \<i>\<s> R * { mk (1(k := f))}
-\<Longrightarrow> k2 \<in> dom f
-\<Longrightarrow> get res k k2 = f k2\<close>
-  using raw_unit_assertion_implies'[unfolded map_le_def]
-  by simp
-
-end
-
-subsubsection \<open>Permission Fiction\<close>
-
-locale share_fiction_for_partial_mapping_resource2 =
-  R: partial_map_resource2 Res
-  +  fiction_kind FIC.DOMAIN INTERPRET Fic \<open>R.share_fiction\<close>
-  for Res :: "('key \<Rightarrow> 'key2 \<Rightarrow> 'val::discrete_semigroup option) resource_entry"
-    and Fic :: "('key \<Rightarrow> 'key2 \<Rightarrow> 'val share option) fiction_entry"
-begin
-
-sublocale permission_fiction Res \<open>R.share_orthogonal_homo\<close> Fic
-  apply (standard, instantiate UNIV; simp add: pointwise_set_UNIV kernel_is_1_def)
-  using comp_eq_dest_lhs by fastforce
-
-lemma [simp]:
-  \<open>R.share_orthogonal_homo (1(k := f)) = 1(k := to_share o f)\<close>
-  unfolding fun_eq_iff by simp
-
-lemmas partial_implies = partial_implies_raw
-
-lemma partial_implies':
-  \<open> r \<in> FIC.SPACE
-\<Longrightarrow> 0 < n
-\<Longrightarrow> r ## mk (1(k := 1(k2 \<mapsto> Share n v)))
-\<Longrightarrow> \<s>\<t>\<a>\<t>\<e> res \<i>\<s> INTERP (r * mk (1(k := 1(k2 \<mapsto> Share n v))))
-\<Longrightarrow> R.get res k k2 = Some v\<close>
-  using partial_implies_raw[where x=\<open>1(k := 1(k2 \<mapsto> v))\<close> and n=n, simplified]
-    discrete_partial_map_subsumption
-  by (smt (verit, del_insts) fun_upd_same join_sub_def sep_disj_fun_def sep_disj_option_discrete(1) times_fupdt_1_apply_sep times_option(3))
-
-lemma partial_implies'':
-  assumes FS: \<open>r \<in> FIC.SPACE\<close>
-    and N: \<open>0 < n\<close>
-    and S: \<open>r ## mk (1(k := 1(k2 \<mapsto> Share n v)))\<close>
-    and A: \<open> \<s>\<t>\<a>\<t>\<e> res \<i>\<s> INTERP (r * mk (1(k := 1(k2 \<mapsto> Share n v)))) \<close>
-  shows [simp]: \<open>R.get res k k2 = Some v\<close>
-proof -
-  from partial_implies'[OF FS, OF N, OF S, OF A]
-  show ?thesis by fastforce
-qed
-
-end
-
-
-section \<open>Common Instructions\<close>
+  by clarsimp
+
+subsection \<open>Synthesis of Value\<close>
+
+subsubsection \<open>Literal Value\<close>
+
+definition [\<phi>programming_simps]: \<open>literal x \<equiv> x\<close> \<comment> \<open>tagging to synthesis a literal\<close>
+
+declare [[\<phi>reason_default_pattern
+      \<open>?X \<t>\<r>\<a>\<n>\<s>\<f>\<o>\<r>\<m>\<s> ?y \<Ztypecolon> \<v>\<a>\<l>[semantic_literal _] ?T \<r>\<e>\<m>\<a>\<i>\<n>\<s> _ @action synthesis\<close> \<Rightarrow>
+      \<open>?X \<t>\<r>\<a>\<n>\<s>\<f>\<o>\<r>\<m>\<s> ?y \<Ztypecolon> \<v>\<a>\<l>[semantic_literal _] ?T \<r>\<e>\<m>\<a>\<i>\<n>\<s> _ @action synthesis\<close>
+      \<open>?X \<t>\<r>\<a>\<n>\<s>\<f>\<o>\<r>\<m>\<s> ?y \<Ztypecolon> \<v>\<a>\<l>[semantic_literal _]  _ \<r>\<e>\<m>\<a>\<i>\<n>\<s> _ @action synthesis\<close>    (500) ]]
+
+setup \<open>Context.theory_map (
+  Phi_Reasoner.add_pass
+      (Const("Phi_Type_of_Literal.synthesisable_literals", dummyT),
+       \<^pattern_prop>\<open>?X \<t>\<r>\<a>\<n>\<s>\<f>\<o>\<r>\<m>\<s> ?y \<Ztypecolon> \<v>\<a>\<l>[semantic_literal _] ?T \<r>\<e>\<m>\<a>\<i>\<n>\<s> _ @action synthesis\<close>,
+       fn pos => fn (rules, prio, patterns, guard, ctxt) =>
+          let val T_names =
+                     fold ((fn Const(\<^const_name>\<open>REMAINS\<close>, _) $ (
+                                  Const(\<^const_name>\<open>\<phi>Type\<close>, _) $ _
+                                    $ (Const(\<^const_name>\<open>Val\<close>, _) $ _ $ T)) $ _ $ _ =>
+                                 (case Term.head_of T
+                                    of Const(N, _) => insert (op =) N
+                                     | _ => I)
+                             | _ => I)
+                           o #2 o Phi_Syntax.dest_transformation o Thm.concl_of) rules []
+           in if null T_names then ()
+                 else Synchronized.change Phi_Type_of_Literal.synthesisable_literals
+                                          (fold Symtab.insert_set T_names);
+              (rules, prio, patterns, guard, ctxt)
+          end
+       )
+)\<close>
+
+lemma "_synthesis_literal_":
+  \<open> R \<t>\<r>\<a>\<n>\<s>\<f>\<o>\<r>\<m>\<s> const \<Ztypecolon> \<v>\<a>\<l>[semantic_literal v] T \<r>\<e>\<m>\<a>\<i>\<n>\<s> R' @action synthesis
+\<Longrightarrow> \<p>\<r>\<o>\<c> Return (semantic_literal v) \<lbrace> R \<longmapsto> \<lambda>ret. const \<Ztypecolon> \<v>\<a>\<l>[ret] T \<r>\<e>\<m>\<a>\<i>\<n>\<s> R' \<rbrace> @action synthesis\<close>
+  unfolding Action_Tag_def Premise_def \<phi>Procedure_def det_lift_def Return_def semantic_literal_def Transformation_def
+  by (clarsimp simp add: Val.unfold INTERP_SPEC_subj Subjection_expn_set INTERP_SPEC, blast)
+
+lemmas [\<phi>reason %\<phi>synthesis_literal] = "_synthesis_literal_"[where const=\<open>literal x\<close> for x]
+
+lemma [\<phi>reason %is_literal]:
+  \<open> Is_Literal (literal x) \<close>
+  unfolding Is_Literal_def ..
+
+
+
+subsubsection \<open>Value Sequence\<close>
+
+lemma semantic_cons_lval_\<phi>app:
+  \<open> \<p>\<r>\<o>\<c> Return (\<phi>V_cons v\<^sub>h v\<^sub>L) \<lbrace> x\<^sub>h \<Ztypecolon> \<v>\<a>\<l>[v\<^sub>h] T\<heavy_comma> x\<^sub>L \<Ztypecolon> \<v>\<a>\<l>\<s>[v\<^sub>L] L \<longmapsto> \<lambda>ret. (x\<^sub>h, x\<^sub>L) \<Ztypecolon> \<v>\<a>\<l>\<s>[ret] (List_Item T \<^emph> L) \<rbrace> \<close>
+  unfolding Premise_def \<phi>Procedure_def det_lift_def Return_def
+  by (cases v\<^sub>h; cases v\<^sub>L; clarsimp simp add: Val.unfold Vals.unfold times_list_def,
+      smt (verit, best) INTERP_SPEC_0(2) Subjection_Flase append_Cons append_self_conv2 empty_iff zero_set_def)
+
+lemma semantic_cons_lval\<^sub>1_\<phi>app:
+  \<open> \<p>\<r>\<o>\<c> Return (\<phi>V_cons v \<phi>V_nil) \<lbrace> x \<Ztypecolon> \<v>\<a>\<l>[v] T \<longmapsto> \<lambda>ret. x \<Ztypecolon> \<v>\<a>\<l>\<s>[ret] List_Item T \<rbrace> \<close>
+  unfolding Premise_def \<phi>Procedure_def det_lift_def Return_def
+  by (cases v; clarsimp simp add: Val.unfold Vals.unfold times_list_def)
+
+
+proc (nodef) [\<phi>reason %\<phi>synthesis_cut
+                  for \<open>\<p>\<r>\<o>\<c> _ \<lbrace> _ \<longmapsto> \<lambda>ret. (_, _) \<Ztypecolon> \<v>\<a>\<l>\<s>[ret] (List_Item _ \<^emph> _) \<r>\<e>\<m>\<a>\<i>\<n>\<s> _ \<rbrace> @action synthesis\<close>]:
+  requires C1: \<open>\<p>\<r>\<o>\<c> C\<^sub>1 \<lbrace> R\<^sub>0 \<longmapsto> \<lambda>ret. x\<^sub>h \<Ztypecolon> \<v>\<a>\<l>[ret] T \<r>\<e>\<m>\<a>\<i>\<n>\<s> R\<^sub>1 \<rbrace> @action synthesis\<close>
+       and C2: \<open>\<p>\<r>\<o>\<c> C\<^sub>2 \<lbrace> R\<^sub>1 \<longmapsto> \<lambda>ret. x\<^sub>L \<Ztypecolon> \<v>\<a>\<l>\<s>[ret] L \<r>\<e>\<m>\<a>\<i>\<n>\<s> R\<^sub>2 \<rbrace> @action synthesis\<close>
+  input  \<open>R\<^sub>0\<close>
+  output \<open>\<lambda>ret. (x\<^sub>h, x\<^sub>L) \<Ztypecolon> \<v>\<a>\<l>\<s>[ret] (List_Item T \<^emph> L) \<r>\<e>\<m>\<a>\<i>\<n>\<s> R\<^sub>2\<close>
+  @action synthesis
+\<medium_left_bracket>
+  C1 C2 semantic_cons_lval
+\<medium_right_bracket> .
+
+
+proc (nodef) [\<phi>reason %\<phi>synthesis_cut
+                  for \<open>\<p>\<r>\<o>\<c> _ \<lbrace> _ \<longmapsto> \<lambda>ret. _ \<Ztypecolon> \<v>\<a>\<l>\<s>[ret] (List_Item _) \<r>\<e>\<m>\<a>\<i>\<n>\<s> _ \<rbrace> @action synthesis\<close>]:
+  requires C: \<open>\<p>\<r>\<o>\<c> C \<lbrace> R\<^sub>0 \<longmapsto> \<lambda>ret. x\<^sub>h \<Ztypecolon> \<v>\<a>\<l>[ret] T \<r>\<e>\<m>\<a>\<i>\<n>\<s> R\<^sub>1 \<rbrace> @action synthesis\<close>
+  input  \<open>R\<^sub>0\<close>
+  output \<open>\<lambda>ret. x\<^sub>h \<Ztypecolon> \<v>\<a>\<l>\<s>[ret] List_Item T \<r>\<e>\<m>\<a>\<i>\<n>\<s> R\<^sub>1\<close>
+  @action synthesis
+\<medium_left_bracket>
+  C semantic_cons_lval\<^sub>1
+\<medium_right_bracket> .
+
+lemma [\<phi>reason %\<phi>synthesis_cut
+           for \<open>\<p>\<r>\<o>\<c> _ \<lbrace> _ \<longmapsto> \<lambda>ret. () \<Ztypecolon> \<v>\<a>\<l>\<s>[ret] \<circle> \<r>\<e>\<m>\<a>\<i>\<n>\<s> _ \<rbrace> @action synthesis\<close>]:
+  \<open> \<p>\<r>\<o>\<c> Return \<phi>V_nil \<lbrace> R\<^sub>0 \<longmapsto> \<lambda>ret. () \<Ztypecolon> \<v>\<a>\<l>\<s>[ret] \<circle> \<r>\<e>\<m>\<a>\<i>\<n>\<s> R\<^sub>0 \<rbrace> \<close>
+  unfolding Premise_def \<phi>Procedure_def det_lift_def Return_def
+  by (clarsimp simp add: Val.unfold Vals.unfold times_list_def)
+
+
+
+
 
 subsection \<open>Drop & Duplicate Value\<close>
 
 lemma [\<phi>reason 1200 for \<open>?x \<Ztypecolon> Val ?raw ?T \<t>\<r>\<a>\<n>\<s>\<f>\<o>\<r>\<m>\<s> ?Y \<w>\<i>\<t>\<h> ?P @action action_dup\<close>]:
   \<open>x \<Ztypecolon> Val raw T \<t>\<r>\<a>\<n>\<s>\<f>\<o>\<r>\<m>\<s> x \<Ztypecolon> Val raw T \<heavy_comma> x \<Ztypecolon> Val raw T @action action_dup\<close>
   unfolding Transformation_def Action_Tag_def
-  by (clarsimp simp add: \<phi>expns)
+  by (clarsimp simp add: Val.unfold INTERP_SPEC Satisfaction_def Subjection_expn_set)
 
 lemma [\<phi>reason 1200 for \<open>?R \<heavy_comma> ?x \<Ztypecolon> Val ?raw ?T \<t>\<r>\<a>\<n>\<s>\<f>\<o>\<r>\<m>\<s> ?Y \<w>\<i>\<t>\<h> ?P @action action_drop\<close>]:
   \<open>Void \<heavy_comma> x \<Ztypecolon> Val raw T \<t>\<r>\<a>\<n>\<s>\<f>\<o>\<r>\<m>\<s> Void @action action_drop\<close>
   unfolding Transformation_def Action_Tag_def
-  by (clarsimp simp add: \<phi>expns)
+  by (clarsimp simp add: Val.unfold)
 
 
 subsection \<open>Abnormal\<close>
@@ -1251,16 +274,17 @@ lemma throw_reduce_tail[procedure_simps,simp]:
 lemma "__throw_rule__"[intro!]:
   \<open> (\<And>a. X a \<t>\<r>\<a>\<n>\<s>\<f>\<o>\<r>\<m>\<s> X' a)
 \<Longrightarrow> \<p>\<r>\<o>\<c> (throw excep :: 'ret proc) \<lbrace> X excep \<longmapsto> Any \<rbrace> \<t>\<h>\<r>\<o>\<w>\<s> X'\<close>
-  unfolding \<phi>Procedure_def subset_iff det_lift_def throw_def Transformation_def Satisfaction_def
-  apply clarsimp
-  by (metis INTERP_SPEC set_mult_expn)
+  unfolding \<phi>Procedure_def subset_iff det_lift_def throw_def Transformation_def
+  by (clarsimp simp add: INTERP_SPEC; metis)
 
 lemma throw_\<phi>app:
-  \<open> (\<And>v. Remove_Values (X v) (X' v))
-\<Longrightarrow> \<p>\<r>\<o>\<c> throw excep \<lbrace> X excep \<longmapsto> 0 \<rbrace> \<t>\<h>\<r>\<o>\<w>\<s> X' \<close>
-  unfolding \<phi>Procedure_def subset_iff det_lift_def throw_def Remove_Values_def Transformation_def Satisfaction_def
-  apply clarsimp
-  by (metis INTERP_SPEC set_mult_expn)
+  \<open> \<p>\<a>\<r>\<a>\<m> excep
+\<Longrightarrow> lambda_abstraction excep XX X
+\<Longrightarrow> (\<And>v. Remove_Values (X v) (X' v))
+\<Longrightarrow> \<p>\<r>\<o>\<c> throw excep \<lbrace> XX \<longmapsto> 0 \<rbrace> \<t>\<h>\<r>\<o>\<w>\<s> X' \<close>
+  unfolding \<phi>Procedure_def subset_iff det_lift_def throw_def Remove_Values_def Transformation_def
+            lambda_abstraction_def
+  by (clarsimp simp add: INTERP_SPEC, metis)
 
 definition op_try :: "'ret proc \<Rightarrow> (ABNM \<Rightarrow> 'ret proc) \<Rightarrow> 'ret proc"
   where \<open>op_try f g s = \<Union>((\<lambda>y. case y of Success x s' \<Rightarrow> {Success x s'}
@@ -1275,10 +299,10 @@ lemma "__op_try__"[intro!]:
 \<Longrightarrow> \<p>\<r>\<o>\<c> op_try f g \<lbrace> X \<longmapsto> \<lambda>v. Y1 v + Y2 v \<rbrace> \<t>\<h>\<r>\<o>\<w>\<s> E2  \<close>
   unfolding op_try_def \<phi>Procedure_def subset_iff
   apply clarsimp subgoal for comp R x s
-    apply (cases s; simp; cases x; clarsimp simp add: set_mult_expn INTERP_SPEC ring_distribs)
+    apply (cases s; simp; cases x; clarsimp simp add: INTERP_SPEC set_mult_expn ring_distribs)
     subgoal premises prems for a b u v
       using prems(1)[THEN spec[where x=comp], THEN spec[where x=R]]
-      by (metis (no_types, lifting) INTERP_SPEC LooseState_expn(1) prems(3) prems(6) prems(7) prems(8) prems(9) set_mult_expn)
+      by (metis (no_types, lifting) INTERP_SPEC LooseState_expn(1) prems(3) prems(6) prems(7) prems(8) prems(9) sep_conj_expn)
     subgoal premises prems for a b c d u v2 proof -
       have \<open>Abnormal a b \<in> LooseState (\<lambda>v. INTERP_SPEC (R \<heavy_comma> Y1 v)) (\<lambda>v. INTERP_SPEC (R \<heavy_comma> E v))\<close>
         using prems(1)[THEN spec[where x=comp], THEN spec[where x=R]]
@@ -1286,10 +310,10 @@ lemma "__op_try__"[intro!]:
       note this[simplified]
       then have \<open>Success c d \<in> LooseState (\<lambda>v. INTERP_SPEC (R \<heavy_comma> Y2 v)) (\<lambda>v. INTERP_SPEC (R \<heavy_comma> E2 v))\<close>
         using prems(2)[of a, THEN spec[where x=b], THEN spec[where x=R]]
-        by (meson INTERP_SPEC prems(4) set_mult_expn)
+        by (meson INTERP_SPEC prems(4) sep_conj_expn)
       note this[simplified]
       then show ?thesis
-        by (metis INTERP_SPEC prems(11) set_mult_expn)
+        by (metis INTERP_SPEC prems(11) sep_conj_expn)
     qed
     subgoal premises prems for a b c d u v proof -
       have \<open>Abnormal a b \<in> LooseState (\<lambda>v. INTERP_SPEC (R \<heavy_comma> Y1 v)) (\<lambda>v. INTERP_SPEC (R \<heavy_comma> E v))\<close>
@@ -1298,13 +322,15 @@ lemma "__op_try__"[intro!]:
       note this[simplified]
       then have \<open>Abnormal c d \<in> LooseState (\<lambda>v. INTERP_SPEC (R \<heavy_comma> Y2 v)) (\<lambda>v. INTERP_SPEC (R \<heavy_comma> E2 v))\<close>
         using prems(2)[THEN spec[where x=b], THEN spec[where x=R]]
-        by (meson INTERP_SPEC prems(4) set_mult_expn)
+        by (meson INTERP_SPEC prems(4) sep_conj_expn)
       note this[simplified]
       then show ?thesis
         by (simp add: INTERP_SPEC set_mult_expn)
     qed
-     apply (smt (z3) INTERP_SPEC LooseState_expn(2) LooseState_expn(3) set_mult_expn)
+     apply (smt (z3) INTERP_SPEC LooseState_expn(2) LooseState_expn(3) sep_conj_expn)
     by blast .
+
+
 
 definition "Union_the_Same_Or_Arbitrary_when_Var Z X Y \<longleftrightarrow> (\<forall>v. (Z::'v \<Rightarrow> 'a set) v = X v + Y v)"
 
@@ -1316,9 +342,8 @@ lemma Union_the_Same_Or_Arbitrary_when_Var__Arbitrary:
   \<open>Union_the_Same_Or_Arbitrary_when_Var (\<lambda>v. X v + Y v) X Y\<close>
   unfolding Union_the_Same_Or_Arbitrary_when_Var_def by blast
 
-\<phi>reasoner_ML Union_the_Same_Or_Arbitrary_when_Var 1200
-  (\<open>Union_the_Same_Or_Arbitrary_when_Var ?Z ?X ?Y\<close>) = \<open>
-fn (ctxt,sequent) =>
+\<phi>reasoner_ML Union_the_Same_Or_Arbitrary_when_Var 1200 (\<open>Union_the_Same_Or_Arbitrary_when_Var ?Z ?X ?Y\<close>) = \<open>
+fn (_, (ctxt,sequent)) =>
   let
     val \<^const>\<open>Trueprop\<close> $ (Const (\<^const_name>\<open>Union_the_Same_Or_Arbitrary_when_Var\<close>, _)
           $ Z $ _ $ _) = Thm.major_prem_of sequent
@@ -1353,527 +378,7 @@ proc (nodef) try':
   \<medium_right_bracket>.
 
 
-subsection \<open>Access the Resource\<close>
 
-subsubsection \<open>Legacy\<close>
 
-definition \<phi>M_get_res :: \<open>(resource \<Rightarrow> 'a) \<Rightarrow> ('a \<Rightarrow> 'ret proc) \<Rightarrow> 'ret proc\<close>
-  where \<open>\<phi>M_get_res R F = (\<lambda>res. F (R res) res)\<close>
-
-definition \<phi>M_get_res_entry :: \<open>(resource \<Rightarrow> ('k \<rightharpoonup> 'a)) \<Rightarrow> 'k \<Rightarrow> ('a \<Rightarrow> 'ret proc) \<Rightarrow> 'ret proc\<close>
-  where \<open>\<phi>M_get_res_entry R k F =
-    \<phi>M_get_res R (\<lambda>res. case res k of Some v \<Rightarrow> F v | _ \<Rightarrow> (\<lambda>_. {Invalid}))\<close>
-
-definition \<phi>M_set_res :: \<open> (('x \<Rightarrow> 'x) \<Rightarrow> resource \<Rightarrow> resource) \<Rightarrow> ('x \<Rightarrow> 'x) \<Rightarrow> unit proc \<close>
-  where \<open>\<phi>M_set_res Updt F = (\<lambda>res. {Success (\<phi>arg ()) (Updt F res)})\<close>
-
-subsubsection \<open>Getters\<close>
-
-paragraph \<open>basic resource\<close>
-
-context resource begin
-
-definition \<phi>R_get_res :: \<open>('T \<Rightarrow> 'ret proc) \<Rightarrow> 'ret proc\<close> \<comment> \<open>depreciated\<close>
-  where \<open>\<phi>R_get_res F = (\<lambda>res. F (get res) res)\<close>
-
-definition \<phi>R_get_res' :: \<open>'T proc\<close> \<comment> \<open>use this\<close>
-  where \<open>\<phi>R_get_res' = (\<lambda>res. Return (\<phi>arg (get res)) res)\<close>
-
-lemma \<phi>R_get_res'_valid:
-  \<open>Valid_Proc \<phi>R_get_res'\<close>
-  unfolding Valid_Proc_def \<phi>R_get_res'_def Return_def det_lift_def
-  by simp
-
-lemma \<phi>R_get_res[intro!]:
-  \<open> get res = v
-\<Longrightarrow> F v res \<r>\<e>\<s>\<u>\<l>\<t>\<s> \<i>\<n> Y \<t>\<h>\<r>\<o>\<w>\<s> E
-\<Longrightarrow> \<phi>R_get_res F res \<r>\<e>\<s>\<u>\<l>\<t>\<s> \<i>\<n> Y \<t>\<h>\<r>\<o>\<w>\<s> E\<close>
-  unfolding \<phi>R_get_res_def subset_iff by simp
-
-end
-
-(* paragraph \<open>discrete_mono_resource\<close>
-
-definition (in discrete_mono_resource) \<phi>R_get_res_entry :: \<open>('T \<Rightarrow> 'ret proc) \<Rightarrow> 'ret proc\<close>
-  where \<open>\<phi>R_get_res_entry F = \<phi>R_get_res (\<lambda>v. case v of Some v' \<Rightarrow> F (discrete.dest v')
-                                                      | _ \<Rightarrow> (\<lambda>_. {Invalid}))\<close>
-
-lemma (in discrete_mono_resource) \<phi>R_get_res_entry:
-  \<open> get res = Some (discrete v)
-\<Longrightarrow> F v res \<r>\<e>\<s>\<u>\<l>\<t>\<s> \<i>\<n> Y \<t>\<h>\<r>\<o>\<w>\<s> E
-\<Longrightarrow> \<phi>R_get_res_entry F res \<r>\<e>\<s>\<u>\<l>\<t>\<s> \<i>\<n> Y \<t>\<h>\<r>\<o>\<w>\<s> E\<close>
-  unfolding \<phi>R_get_res_entry_def \<phi>R_get_res_def by simp *)
-
-paragraph \<open>partial_map_resource\<close>
-
-definition (in partial_map_resource)
-  \<phi>R_get_res_entry :: \<open>'key \<Rightarrow> ('val \<Rightarrow> 'ret proc) \<Rightarrow> 'ret proc\<close>
-  where \<open>\<phi>R_get_res_entry k F =
-    \<phi>R_get_res (\<lambda>res. case res k of Some v \<Rightarrow> F v | _ \<Rightarrow> (\<lambda>_. {Invalid}))\<close>
-
-definition (in partial_map_resource)
-  \<phi>R_get_res_entry' :: \<open>'key \<Rightarrow> 'val proc\<close>
-  where \<open>\<phi>R_get_res_entry' k =
-    \<phi>R_get_res' \<bind> (\<lambda>res. case \<phi>arg.dest res k of Some v \<Rightarrow> Return (\<phi>arg v) | _ \<Rightarrow> (\<lambda>_. {Invalid}))\<close>
-
-lemma (in partial_map_resource) \<phi>R_get_res_entry[intro!]:
-  \<open> get res k = Some v
-\<Longrightarrow> F v res \<r>\<e>\<s>\<u>\<l>\<t>\<s> \<i>\<n> Y \<t>\<h>\<r>\<o>\<w>\<s> E
-\<Longrightarrow> \<phi>R_get_res_entry k F res \<r>\<e>\<s>\<u>\<l>\<t>\<s> \<i>\<n> Y \<t>\<h>\<r>\<o>\<w>\<s> E\<close>
-  unfolding \<phi>R_get_res_entry_def \<phi>R_get_res_def by simp
-
-subparagraph \<open>identity_fiction_for_partial_mapping_resource\<close>
-
-context identity_fiction_for_partial_mapping_resource begin
-
-lemma \<phi>R_get_res_entry_frm[intro!]:
-  \<open>\<p>\<r>\<o>\<c> F v
-      \<lbrace> R\<heavy_comma> v \<Ztypecolon> \<phi> (key \<^bold>\<rightarrow> \<black_circle> Itself) \<longmapsto> Y \<rbrace> \<t>\<h>\<r>\<o>\<w>\<s> E
-\<Longrightarrow> \<p>\<r>\<o>\<c> R.\<phi>R_get_res_entry key F
-      \<lbrace> R\<heavy_comma> v \<Ztypecolon> \<phi> (key \<^bold>\<rightarrow> \<black_circle> Itself) \<longmapsto> Y \<rbrace> \<t>\<h>\<r>\<o>\<w>\<s> E \<close>
-  unfolding \<phi>Procedure_Hybrid_DL \<phi>Res_Spec_expn_R imp_conjL
-            \<phi>Res_Sat_expn_impEx \<phi>Res_Sat_expn_impSubj
-  by (clarsimp simp add: \<phi>expns expand; rule R.\<phi>R_get_res_entry[where v=v]; simp)
-
-lemmas \<phi>R_get_res_entry[intro!] = \<phi>R_get_res_entry_frm[where R=1, simplified]
-
-end
-
-subparagraph \<open>share_fiction_for_partial_mapping_resource\<close>
-
-context share_fiction_for_partial_mapping_resource begin
-
-lemma \<phi>R_get_res_entry_frm[intro!]:
-  \<open>\<p>\<r>\<o>\<c> F v
-      \<lbrace> R\<heavy_comma> v \<Ztypecolon> \<phi> (key \<^bold>\<rightarrow> n \<odiv> \<fish_eye> Itself) \<longmapsto> Y \<rbrace> \<t>\<h>\<r>\<o>\<w>\<s> E
-\<Longrightarrow> \<p>\<r>\<o>\<c> R.\<phi>R_get_res_entry key F
-      \<lbrace> R\<heavy_comma> v \<Ztypecolon> \<phi> (key \<^bold>\<rightarrow> n \<odiv> \<fish_eye> Itself) \<longmapsto> Y \<rbrace> \<t>\<h>\<r>\<o>\<w>\<s> E \<close>
-  unfolding \<phi>Procedure_Hybrid_DL
-    \<phi>Res_Spec_expn_R \<phi>Res_Sat_expn_impEx \<phi>Res_Sat_expn_impSubj imp_conjL
-  apply (clarsimp simp add: \<phi>expns zero_set_def)
-  apply (rule R.\<phi>R_get_res_entry[where v=v])
-  apply simp
-  by blast
-
-lemmas \<phi>R_get_res_entry[intro!] = \<phi>R_get_res_entry_frm[where R=1, simplified]
-
-end
-
-paragraph \<open>partial_map_resource2\<close>
-
-definition (in partial_map_resource2) \<comment> \<open>depreciated\<close>
-    \<phi>R_get_res_entry :: \<open>'key \<Rightarrow> 'key2 \<Rightarrow> ('val \<Rightarrow> 'ret proc) \<Rightarrow> 'ret proc\<close>
-  where \<open>\<phi>R_get_res_entry k k2 F = \<phi>R_get_res (\<lambda>res.
-    case res k k2 of Some v \<Rightarrow> F v | _ \<Rightarrow> (\<lambda>_. {Invalid}))\<close>
-
-definition (in partial_map_resource2)
-  \<phi>R_get_res_entry' :: \<open>'key \<Rightarrow> 'key2 \<Rightarrow> 'val proc\<close>
-  where \<open>\<phi>R_get_res_entry' k k2 =
-    \<phi>R_get_res' \<bind> (\<lambda>res. case \<phi>arg.dest res k k2 of Some v \<Rightarrow> Return (\<phi>arg v) | _ \<Rightarrow> (\<lambda>_. {Invalid}))\<close>
-
-
-lemma (in partial_map_resource2) \<phi>R_get_res_entry[intro!]:
-  \<open> get res k k2 = Some v
-\<Longrightarrow> F v res \<r>\<e>\<s>\<u>\<l>\<t>\<s> \<i>\<n> Y \<t>\<h>\<r>\<o>\<w>\<s> E
-\<Longrightarrow> \<phi>R_get_res_entry k k2 F res \<r>\<e>\<s>\<u>\<l>\<t>\<s> \<i>\<n> Y \<t>\<h>\<r>\<o>\<w>\<s> E\<close>
-  unfolding \<phi>R_get_res_entry_def \<phi>R_get_res_def by simp
-
-lemma (in share_fiction_for_partial_mapping_resource2) \<phi>R_get_res_entry[intro!]:
-  \<open>\<p>\<r>\<o>\<c> F v
-      \<lbrace> v \<Ztypecolon> \<phi> (k1 \<^bold>\<rightarrow> k2 \<^bold>\<rightarrow> n \<odiv> \<fish_eye> Itself) \<longmapsto> Y \<rbrace> \<t>\<h>\<r>\<o>\<w>\<s> E
-\<Longrightarrow> \<p>\<r>\<o>\<c> R.\<phi>R_get_res_entry k1 k2 F
-      \<lbrace> v \<Ztypecolon> \<phi> (k1 \<^bold>\<rightarrow> k2 \<^bold>\<rightarrow> n \<odiv> \<fish_eye> Itself) \<longmapsto> Y \<rbrace> \<t>\<h>\<r>\<o>\<w>\<s> E \<close>
-  unfolding \<phi>Procedure_Hybrid_DL
-  apply (clarsimp simp add: \<phi>expns zero_set_def)
-  apply (rule R.\<phi>R_get_res_entry[where v=v])
-  apply simp
-  by blast
-
-lemma (in share_fiction_for_partial_mapping_resource2) \<phi>R_get_res_entry1[intro!]:
-  \<open>\<p>\<r>\<o>\<c> F v
-      \<lbrace> v \<Ztypecolon> \<phi> (k1 \<^bold>\<rightarrow> k2 \<^bold>\<rightarrow> \<fish_eye> Itself) \<longmapsto> Y \<rbrace> \<t>\<h>\<r>\<o>\<w>\<s> E
-\<Longrightarrow> \<p>\<r>\<o>\<c> R.\<phi>R_get_res_entry k1 k2 F
-      \<lbrace> v \<Ztypecolon> \<phi> (k1 \<^bold>\<rightarrow> k2 \<^bold>\<rightarrow> \<fish_eye> Itself) \<longmapsto> Y \<rbrace> \<t>\<h>\<r>\<o>\<w>\<s> E \<close>
-  using \<phi>R_get_res_entry[where n=1, simplified] .
-
-
-subsubsection \<open>Setters\<close>
-
-definition (in resource) \<phi>R_set_res :: \<open>('T \<Rightarrow> 'T) \<Rightarrow> unit proc\<close>
-  where \<open>\<phi>R_set_res F = (\<lambda>res. {Success (\<phi>arg ()) (updt F res)})\<close>
-
-definition (in resource) \<phi>R_set_res' :: \<open>('T \<Rightarrow> 'T) \<Rightarrow> unit proc\<close>
-  where \<open>\<phi>R_set_res' F = (\<lambda>res. if updt F res \<in> SPACE
-                                then {Success (\<phi>arg ()) (updt F res)}
-                                else {Invalid})\<close>
-
-paragraph \<open>partial_map_resource\<close>
-
-lemma (in partial_map_resource) \<phi>R_set_res:
-  \<open> (\<forall>m. m \<in>\<^sub>S\<^sub>H domain \<longrightarrow> P m \<longrightarrow> m(k := u) \<in>\<^sub>S\<^sub>H domain)
-\<Longrightarrow> P (get res)
-\<Longrightarrow> \<s>\<t>\<a>\<t>\<e> res \<i>\<s> R * {mk (1(k \<mapsto> any))}
-\<Longrightarrow> \<phi>R_set_res (\<lambda>f. f(k := u)) res \<r>\<e>\<s>\<u>\<l>\<t>\<s> \<i>\<n> (\<lambda>_. R * {mk (1(k := u))}) \<t>\<h>\<r>\<o>\<w>\<s> Any\<close>
-  unfolding \<phi>R_set_res_def
-  by (simp add: \<phi>expns "__updt_rule__")
-
-context identity_fiction_for_partial_mapping_resource begin
-
-lemma \<phi>R_set_res:
-  \<open> (\<forall>m. m \<in>\<^sub>S\<^sub>H R.domain \<longrightarrow> P m \<longrightarrow> m(k \<mapsto> u) \<in>\<^sub>S\<^sub>H R.domain)
-\<Longrightarrow> (\<And>res r. (\<s>\<t>\<a>\<t>\<e> res \<i>\<s> INTERP r * {R.mk (1(k \<mapsto> v))}) \<Longrightarrow> P (R.get res))
-\<Longrightarrow> \<p>\<r>\<o>\<c> R.\<phi>R_set_res (\<lambda>f. f(k \<mapsto> u))
-         \<lbrace> v \<Ztypecolon> \<phi> (k \<^bold>\<rightarrow> \<black_circle> Itself) \<longmapsto> \<lambda>\<r>\<e>\<t>. u \<Ztypecolon> \<phi> (k \<^bold>\<rightarrow> \<black_circle> Itself) \<rbrace>\<close>
-  unfolding \<phi>Procedure_Hybrid_DL
-  apply (clarsimp simp add: \<phi>expns zero_set_def
-          expand[where x=\<open>1(k \<mapsto> v)\<close>, simplified]
-          expand_subj[where x=\<open>1(k \<mapsto> u)\<close>, simplified])
-  subgoal for r res
-    thm R.\<phi>R_set_res[where k=k and res=res]
-    by (rule R.\<phi>R_set_res[where k=k and res=res], assumption, simp, assumption) .
-
-declare \<phi>R_set_res[THEN \<phi>CONSEQ'E0, intro!]
-lemmas \<phi>R_set_res_frm[intro!] = \<phi>R_set_res[THEN \<phi>frame, simplified, THEN \<phi>CONSEQ'E0[simplified zero_fun_def]]
-end
-
-context share_fiction_for_partial_mapping_resource begin
-
-lemma \<phi>R_set_res:
-  \<open> (\<forall>m. m \<in>\<^sub>S\<^sub>H R.domain \<longrightarrow> P m \<longrightarrow> m(k \<mapsto> u) \<in>\<^sub>S\<^sub>H R.domain)
-\<Longrightarrow> (\<And>res r. \<s>\<t>\<a>\<t>\<e> res \<i>\<s> INTERP r * {R.mk (1(k \<mapsto> v))} \<Longrightarrow> P (R.get res))
-\<Longrightarrow> \<p>\<r>\<o>\<c> R.\<phi>R_set_res (\<lambda>f. f(k \<mapsto> u))
-         \<lbrace> v \<Ztypecolon> \<phi> (k \<^bold>\<rightarrow> \<fish_eye> Itself) \<longmapsto> \<lambda>\<r>\<e>\<t>. u \<Ztypecolon> \<phi> (k \<^bold>\<rightarrow> \<fish_eye> Itself) \<rbrace>\<close>
-  unfolding \<phi>Procedure_Hybrid_DL
-  apply (clarsimp simp add: \<phi>expns zero_set_def
-          expand[where x=\<open>1(k \<mapsto> v)\<close>, simplified]
-          expand_subj[where x=\<open>1(k \<mapsto> u)\<close>, simplified])
-  subgoal for r res
-    by (rule R.\<phi>R_set_res[where k=k and res=res], assumption, simp, assumption) .
-
-declare \<phi>R_set_res[THEN \<phi>CONSEQ'E0, intro!]
-lemmas \<phi>R_set_res_frm[intro!] = \<phi>R_set_res[THEN \<phi>frame, simplified, THEN \<phi>CONSEQ'E0[simplified zero_fun_def]]
-
-end
-
-
-paragraph \<open>partial_map_resource2\<close>
-
-lemma (in partial_map_resource2) \<phi>R_set_res[intro!]:
-  \<open> (\<forall>m. m \<in>\<^sub>S\<^sub>H domain \<longrightarrow> P m \<longrightarrow> map_fun_at (map_fun_at (\<lambda>_. u) k2) k m \<in>\<^sub>S\<^sub>H domain)
-\<Longrightarrow> P (get res)
-\<Longrightarrow> \<s>\<t>\<a>\<t>\<e> res \<i>\<s> R * {mk (1(k := 1(k2 \<mapsto> any)))}
-\<Longrightarrow> \<phi>R_set_res (map_fun_at (map_fun_at (\<lambda>_. u) k2) k) res
-      \<r>\<e>\<s>\<u>\<l>\<t>\<s> \<i>\<n> (\<lambda>_. R * {mk (1(k := 1(k2 := u)))}) \<t>\<h>\<r>\<o>\<w>\<s> Any\<close>
-  unfolding \<phi>R_set_res_def by (simp add: \<phi>expns "__updt_rule__")
-
-lemma (in share_fiction_for_partial_mapping_resource2) "\<phi>R_set_res"[THEN \<phi>CONSEQ'E0, intro!]:
-  \<open> (\<forall>m. m \<in>\<^sub>S\<^sub>H R.domain \<longrightarrow> P m \<longrightarrow> (map_fun_at (map_fun_at (\<lambda>_. Some u) k2) k) m \<in>\<^sub>S\<^sub>H R.domain)
-\<Longrightarrow> (\<And>res r. \<s>\<t>\<a>\<t>\<e> res \<i>\<s> INTERP r * {R.mk (1(k := 1(k2 \<mapsto> v)))} \<Longrightarrow> P (R.get res))
-\<Longrightarrow> \<p>\<r>\<o>\<c> R.\<phi>R_set_res (map_fun_at (map_fun_at (\<lambda>_. Some u) k2) k)
-         \<lbrace> v \<Ztypecolon> \<phi> (k \<^bold>\<rightarrow> k2 \<^bold>\<rightarrow> \<fish_eye> Itself) \<longmapsto> \<lambda>\<r>\<e>\<t>. u \<Ztypecolon> \<phi> (k \<^bold>\<rightarrow> k2 \<^bold>\<rightarrow> \<fish_eye> Itself) \<rbrace>\<close>
-  unfolding \<phi>Procedure_Hybrid_DL
-  apply (clarsimp simp add: \<phi>expns zero_set_def
-                            expand[where x=\<open>1(k := 1(k2 \<mapsto> v))\<close>, simplified]
-                            expand_subj[where x=\<open>1(k := 1(k2 \<mapsto> u))\<close>, simplified])
-  subgoal for r res
-    by (rule R.\<phi>R_set_res, assumption, simp, assumption) .
-
-
-subsubsection \<open>Dispose\<close>
-
-paragraph \<open>partial_map_resource\<close>
-
-lemma (in partial_map_resource) \<phi>R_dispose_res[intro!]:
-  \<open> (\<forall>m. m \<in>\<^sub>S\<^sub>H domain \<longrightarrow> P m \<longrightarrow> m(k := None) \<in>\<^sub>S\<^sub>H domain)
-\<Longrightarrow> P (get res)
-\<Longrightarrow> \<s>\<t>\<a>\<t>\<e> res \<i>\<s> R * {mk (1(k \<mapsto> any))}
-\<Longrightarrow> \<phi>R_set_res (\<lambda>f. f(k := None)) res \<r>\<e>\<s>\<u>\<l>\<t>\<s> \<i>\<n> (\<lambda>_. R) \<t>\<h>\<r>\<o>\<w>\<s> Any\<close>
-  unfolding \<phi>R_set_res_def by (simp add: \<phi>expns "__dispose_rule__")
-
-context identity_fiction_for_partial_mapping_resource begin
-
-lemma \<phi>R_dispose_res:
-  \<open> (\<forall>m. m \<in>\<^sub>S\<^sub>H R.domain \<longrightarrow> P m \<longrightarrow> m(k := None) \<in>\<^sub>S\<^sub>H R.domain)
-\<Longrightarrow> (\<And>res r. \<s>\<t>\<a>\<t>\<e> res \<i>\<s> INTERP r * {R.mk (1(k \<mapsto> v))} \<Longrightarrow> P (R.get res))
-\<Longrightarrow> \<p>\<r>\<o>\<c> R.\<phi>R_set_res (\<lambda>f. f(k := None))
-         \<lbrace> v \<Ztypecolon> \<phi> (k \<^bold>\<rightarrow> \<black_circle> Itself) \<longmapsto> \<lambda>_. Void \<rbrace>\<close>
-  unfolding \<phi>Procedure_Hybrid_DL
-  apply (clarsimp simp add: \<phi>expns zero_set_def expand[where x=\<open>1(k \<mapsto> v)\<close>, simplified])
-  subgoal for r res
-    by (rule R.\<phi>R_dispose_res, assumption, simp, simp) .
-
-declare \<phi>R_dispose_res[THEN \<phi>CONSEQ'E0, intro!]
-lemmas \<phi>R_dispose_res_frm[intro!] = \<phi>R_dispose_res[THEN \<phi>frame, simplified, THEN \<phi>CONSEQ'E0[simplified zero_fun_def]]
-
-end
-
-context share_fiction_for_partial_mapping_resource begin
-
-lemma \<phi>R_dispose_res:
-  \<open> (\<forall>m. m \<in>\<^sub>S\<^sub>H R.domain \<longrightarrow> P m \<longrightarrow> m(k := None) \<in>\<^sub>S\<^sub>H R.domain)
-\<Longrightarrow> (\<And>res r. \<s>\<t>\<a>\<t>\<e> res \<i>\<s> INTERP r * {R.mk (1(k \<mapsto> v))} \<Longrightarrow> P (R.get res))
-\<Longrightarrow> \<p>\<r>\<o>\<c> R.\<phi>R_set_res (\<lambda>f. f(k := None))
-         \<lbrace> v \<Ztypecolon> \<phi> (k \<^bold>\<rightarrow> \<fish_eye> Itself) \<longmapsto> \<lambda>_. Void \<rbrace>\<close>
-  unfolding \<phi>Procedure_Hybrid_DL
-  apply (clarsimp simp add: \<phi>expns zero_set_def expand[where x=\<open>1(k \<mapsto> v)\<close>, simplified])
-  subgoal for r res by (rule R.\<phi>R_dispose_res, assumption, simp, simp) .
-
-declare \<phi>R_dispose_res[THEN \<phi>CONSEQ'E0, intro!]
-lemmas \<phi>R_dispose_res_frm[intro!] = \<phi>R_dispose_res[THEN \<phi>frame, simplified, THEN \<phi>CONSEQ'E0[simplified zero_fun_def]]
-
-end
-
-paragraph \<open>partial_map_resource2\<close>
-
-lemma (in partial_map_resource2) \<phi>R_dispose_res[intro!]:
-  \<open> (\<forall>m. m \<in>\<^sub>S\<^sub>H domain \<longrightarrow> P m \<longrightarrow> m(k:=1) \<in>\<^sub>S\<^sub>H domain)
-\<Longrightarrow> dom (get res k) = dom any
-\<Longrightarrow> P (get res)
-\<Longrightarrow> \<s>\<t>\<a>\<t>\<e> res \<i>\<s> R * {mk (1(k := any))}
-\<Longrightarrow> \<phi>R_set_res (\<lambda>f. f(k := 1)) res \<r>\<e>\<s>\<u>\<l>\<t>\<s> \<i>\<n> (\<lambda>_. R) \<t>\<h>\<r>\<o>\<w>\<s> Any\<close>
-  unfolding \<phi>R_set_res_def by (simp add: \<phi>expns "__dispose_rule__")
-
-lemma (in share_fiction_for_partial_mapping_resource2) "\<phi>R_dispose_res"[THEN \<phi>CONSEQ'E0, intro!]:
-  \<open> (\<forall>m. m \<in>\<^sub>S\<^sub>H R.domain \<longrightarrow> P m \<longrightarrow> m(k := 1) \<in>\<^sub>S\<^sub>H R.domain)
-\<Longrightarrow> (\<And>res r. \<s>\<t>\<a>\<t>\<e> res \<i>\<s> INTERP r * {R.mk (1(k := f))}
-      \<Longrightarrow> P (R.get res) \<and> dom f = dom (R.get res k))
-\<Longrightarrow> \<p>\<r>\<o>\<c> R.\<phi>R_set_res (\<lambda>f. f(k := 1))
-         \<lbrace> to_share o f \<Ztypecolon> \<phi> (k \<^bold>\<rightarrow> Itself) \<longmapsto> \<lambda>_. Void \<rbrace>\<close>
-  unfolding \<phi>Procedure_Hybrid_DL
-  apply (clarsimp simp add: \<phi>expns zero_set_def expand[where x=\<open>1(k := f)\<close>, simplified])
-  subgoal for r res
-    apply (rule R.\<phi>R_dispose_res, assumption, standard, simp)
-    subgoal premises prems proof -
-      have t1: \<open>dom f = dom (R.get res k)\<close>
-        using prems(2) prems(3) by blast
-      have t2: \<open>f \<subseteq>\<^sub>m R.get res k\<close>
-        using R.raw_unit_assertion_implies' prems(3) by blast
-      have t3: \<open>R.get res k = f\<close>
-        by (metis (no_types, lifting) map_le_antisym map_le_def t1 t2)
-      show ?thesis
-        using prems(3) t3 by blast
-    qed . .
-
-subsubsection \<open>Allocate\<close>
-
-context mapping_resource begin
-
-definition
-    \<phi>R_allocate_res_entry :: \<open>('key \<Rightarrow> bool)
-                           \<Rightarrow> 'val
-                           \<Rightarrow> ('key \<Rightarrow> 'ret proc)
-                           \<Rightarrow> 'ret proc\<close>
-  where \<open>\<phi>R_allocate_res_entry P init F =
-    \<phi>R_get_res (\<lambda>res.
-    let k = (@k. res k = 1 \<and> P k)
-     in \<phi>R_set_res (\<lambda>f. f(k := init))
-        \<ggreater> F k
-)\<close>
-
-definition
-    \<phi>R_allocate_res_entry' :: \<open>('key \<Rightarrow> bool)
-                           \<Rightarrow> 'val
-                           \<Rightarrow> 'key proc\<close>
-  where \<open>\<phi>R_allocate_res_entry' P init =
-    \<phi>R_get_res (\<lambda>res.
-    let k = (@k. res k = 1 \<and> P k)
-     in \<phi>R_set_res (\<lambda>f. f(k := init))
-        \<ggreater> Return (\<phi>arg k)
-)\<close>
-
-lemma \<phi>R_set_res_new[intro!]:
-  \<open> (\<forall>m. m \<in>\<^sub>S\<^sub>H domain \<longrightarrow> m(k := u) \<in>\<^sub>S\<^sub>H domain)
-\<Longrightarrow> k \<notin> dom1 (get res)
-\<Longrightarrow> \<s>\<t>\<a>\<t>\<e> res \<i>\<s> R
-\<Longrightarrow> \<phi>R_set_res (\<lambda>f. f(k := u)) res \<r>\<e>\<s>\<u>\<l>\<t>\<s> \<i>\<n> (\<lambda>_. R * {mk (1(k := u))}) \<t>\<h>\<r>\<o>\<w>\<s> Any\<close>
-  unfolding \<phi>R_set_res_def
-  by (simp add: \<phi>expns "__allocation_rule__")
-
-lemma \<phi>R_allocate_res_entry[intro!]:
-  \<open> (\<forall>m. m \<in>\<^sub>S\<^sub>H domain \<longrightarrow> (\<exists>k. m k = 1 \<and> P k))
-\<Longrightarrow> (\<forall>k m. P k \<longrightarrow> m \<in>\<^sub>S\<^sub>H domain \<longrightarrow> m(k := init) \<in>\<^sub>S\<^sub>H domain)
-\<Longrightarrow> (\<And>k res. \<s>\<t>\<a>\<t>\<e> res \<i>\<s> R * {mk (1(k := init))} \<s>\<u>\<b>\<j> P k
-      \<Longrightarrow> F k res \<r>\<e>\<s>\<u>\<l>\<t>\<s> \<i>\<n> Y \<t>\<h>\<r>\<o>\<w>\<s> E)
-\<Longrightarrow> \<s>\<t>\<a>\<t>\<e> res \<i>\<s> R
-\<Longrightarrow> \<phi>R_allocate_res_entry P init F res \<r>\<e>\<s>\<u>\<l>\<t>\<s> \<i>\<n> Y \<t>\<h>\<r>\<o>\<w>\<s> E\<close>
-  unfolding \<phi>R_allocate_res_entry_def \<phi>R_get_res_def
-  subgoal premises prems proof -
-    let ?m = \<open>get res\<close>
-    define k' where \<open>k' = (SOME k. ?m k = 1 \<and> P k)\<close>
-    have \<open>\<exists>k'. ?m k' = 1 \<and> P k'\<close>
-      using get_res_Valid prems(1) prems(4) by blast
-    note this[THEN someI_ex]
-    then have t1[simp]: \<open>?m k' = 1 \<and> P k'\<close> unfolding k'_def by blast
-    show ?thesis
-      unfolding k'_def[symmetric]
-      apply (simp, rule \<phi>M_RS_WP_SEQ, rule \<phi>R_set_res_new)
-      using prems(2) t1 apply blast
-      apply (simp add: dom1_def)
-      using \<open>\<s>\<t>\<a>\<t>\<e> res \<i>\<s> _\<close> apply this
-      by (simp add: prems(3))
-  qed .
-
-end
-
-lemma (in identity_fiction_for_partial_mapping_resource) "\<phi>R_allocate_res_entry"[intro!]:
-  \<open> (\<forall>m. m \<in>\<^sub>S\<^sub>H R.domain \<longrightarrow> (\<exists>k. m k = 1 \<and> P k))
-\<Longrightarrow> (\<forall>k m. P k \<longrightarrow> m \<in>\<^sub>S\<^sub>H R.domain \<longrightarrow> m(k \<mapsto> init) \<in>\<^sub>S\<^sub>H R.domain)
-\<Longrightarrow> (\<And>new. P new \<Longrightarrow> \<p>\<r>\<o>\<c> F new \<lbrace> X \<heavy_comma> init \<Ztypecolon> \<phi> (new \<^bold>\<rightarrow> \<black_circle> Itself) \<longmapsto> Y \<rbrace> \<t>\<h>\<r>\<o>\<w>\<s> E)
-\<Longrightarrow> \<p>\<r>\<o>\<c> R.\<phi>R_allocate_res_entry P (Some init) F \<lbrace> X \<longmapsto> Y \<rbrace> \<t>\<h>\<r>\<o>\<w>\<s> E\<close>
- apply (clarsimp simp add: \<phi>expns \<phi>Procedure_Hybrid_DL)
-  subgoal for r res c
-  apply (rule R.\<phi>R_allocate_res_entry[where R="(INTERP (r * c))"])
-  apply (clarsimp)
-  apply (clarsimp)
-  apply (clarsimp)
-  subgoal premises prems for k res'
-  apply (rule prems(3)[OF \<open>P _\<close>, THEN spec[where x=r], THEN spec[where x=res'],
-              simplified prems, simplified, THEN mp])
-    apply (rule exI[where x=\<open>c * mk (1(k \<mapsto> init))\<close>])
-    apply rule
-    apply (smt (verit, ccfv_threshold) SPACE_mult_homo expand prems(6) prems(7) prems(8) prems(9) sep_disj_commute sep_disj_fiction sep_disj_multD2 sep_mult_commute sep_mult_left_commute)
-    apply rule
-    using FIC.SPACE_mult_homo prems(5) prems(6) prems(7) prems(8) prems(9) sep_disj_fiction sep_disj_multD2 apply blast
-    by (metis Fic_Space_m SPACE_mult_homo identity_fiction.sep_disj_fiction identity_fiction_axioms prems(6) prems(7) prems(8) prems(9) sep_disj_multD2 sep_disj_multI2)
-  . .
-
-
-
-(*
-
-
-(*
-subsection \<open>Tuple Operations\<close>
-
-
-
-subsubsection \<open>Construct Tuple\<close>
-
-definition cons_tup :: "TY list \<Rightarrow> VAL list \<Rightarrow> (VAL,'RES_N,'RES) proc"
-  where "cons_tup tys vs = (
-    let N = length tys in
-    \<phi>M_assert (N \<le> length vs \<and> list_all2 (\<lambda>v t. v \<in> Well_Type t) (rev (take N vs)) tys)
-    \<ggreater> Success (V_tup.mk (rev (take N vs))))"
-
-lemma cons_tup_nil:
-  \<open>cons_tup [] = \<phi>M_put_Val (V_tup.mk [])\<close>
-  unfolding cons_tup_def \<phi>M_put_Val_def
-  by simp
-
-lemma cons_tup_cons:
-  \<open>cons_tup (TY#TYs) =
-    cons_tup TYs \<ggreater>
-    \<phi>M_get_Val (\<lambda>tup.
-    \<phi>M_get_Val (\<lambda>v.
-    \<phi>M_assert (v \<in> Well_Type TY) \<ggreater>
-    \<phi>M_put_Val (V_tup.mk [v] * tup)
-    ))\<close>
-  apply (auto split: list.split
-    simp add: cons_tup_def fun_eq_iff pair_forall instr_comp_def bind_def
-    \<phi>M_get_Val_def \<phi>M_assert_def \<phi>M_put_Val_def Let_def V_tup_mult)
-  apply (metis Suc_le_eq list.sel(1) take_hd_drop)
-  apply (metis Cons_nth_drop_Suc Suc_le_eq list.sel(3))
-  apply (metis Suc_le_eq drop_all leI list.simps(3))
-  apply (metis (no_types, lifting) drop_all leI list.ctr_transfer(1) list.sel(1) list.simps(3) list_all2_Cons2 list_all2_appendI list_all2_rev1 rev.simps(2) take_hd_drop)
-  apply (smt (verit, del_insts) Suc_le_eq append1_eq_conv list.sel(1) list_all2_Cons2 rev_eq_Cons_iff take_hd_drop)
-  by (simp add: take_Suc_conv_app_nth)
-
-lemma (in \<phi>empty) op_cons_tup_nil:
-  \<open> \<p>\<r>\<o>\<c> cons_tup [] \<lbrace> Void \<longmapsto> () \<Ztypecolon> EmptyTuple \<rbrace>\<close>
-  unfolding cons_tup_nil by \<phi>reason
-
-lemma (in \<phi>empty) op_cons_tup_cons:
-  \<open> \<p>\<r>\<o>\<c> cons_tup TYs \<lbrace> X \<longmapsto> VAL y \<Ztypecolon> Y \<rbrace>
-\<Longrightarrow> \<phi>SemType (a \<Ztypecolon> A) TY
-\<Longrightarrow> \<p>\<r>\<o>\<c> cons_tup (TY#TYs) \<lbrace> VAL a \<Ztypecolon> A\<heavy_comma> X \<longmapsto> VAL (a,y) \<Ztypecolon> (\<clubsuit> A \<^emph> Y) \<rbrace>\<close>
-  unfolding cons_tup_cons
-  apply \<phi>reason apply (rule \<phi>frame0, assumption)
-  apply \<phi>reason apply (simp add: \<phi>SemType_def subset_iff)
-  apply \<phi>reason apply (simp add: \<phi>expns) by blast
-
-
-subsubsection \<open>Destruct Tuple\<close>
-
-
-definition op_dest_tup :: "TY list \<Rightarrow> (VAL,'RES_N,'RES) proc"
-  where "op_dest_tup tys =
-    \<phi>M_getV (\<tau>Tuple tys) V_tup.dest (\<lambda>tup.
-    \<lambda>(vs, res). Success (rev tup@vs, res))"
-
-lemma op_dest_tup_nil_expn:
-  \<open>op_dest_tup [] = \<phi>M_getV (\<tau>Tuple []) V_tup.dest (\<lambda>_. SKIP)\<close>
-  by (auto split: list.split
-    simp add: op_dest_tup_def \<phi>M_get_Val_def \<phi>M_put_Val_def \<phi>M_getV_def Let_def fun_eq_iff \<phi>M_assert_def
-      instr_comp_def bind_def)
-
-lemma op_dest_tup_cons_expn:
-  \<open>op_dest_tup (TY#TYs) =
-    \<phi>M_get_Val (\<lambda>tup.
-    \<phi>M_assert (\<exists>h tup'. tup = V_tup.mk (h#tup') \<and> h \<in> Well_Type TY) \<ggreater>
-    \<phi>M_put_Val (hd (V_tup.dest tup)) \<ggreater>
-    \<phi>M_put_Val (V_tup.mk (tl (V_tup.dest tup))) \<ggreater>
-    op_dest_tup TYs)\<close>
-  apply (auto split: list.split
-    simp add: op_dest_tup_def \<phi>M_get_Val_def \<phi>M_put_Val_def \<phi>M_getV_def Let_def fun_eq_iff \<phi>M_assert_def
-      instr_comp_def bind_def)
-  by (metis list.discI list.exhaust_sel list.rel_sel list.sel(1))
-
-lemma (in \<phi>empty) op_dest_tup_nil:
-  \<open>\<p>\<r>\<o>\<c> op_dest_tup [] \<lbrace> () \<Ztypecolon> EmptyTuple \<longmapsto> Void \<rbrace> \<close>
-  unfolding op_dest_tup_nil_expn by \<phi>reason
-
-lemma (in \<phi>empty) op_dest_tup_cons:
-  \<open> \<p>\<r>\<o>\<c> op_dest_tup TYs \<lbrace> VAL y \<Ztypecolon> Y \<longmapsto> X \<rbrace>
-\<Longrightarrow> \<phi>SemType (a \<Ztypecolon> A) TY
-\<Longrightarrow> \<p>\<r>\<o>\<c> op_dest_tup (TY#TYs) \<lbrace> VAL (a,y) \<Ztypecolon> (\<clubsuit> A \<^emph> \<phi>Is_Tuple Y) \<longmapsto> VAL a \<Ztypecolon> A\<heavy_comma> X \<rbrace>\<close>
-  unfolding op_dest_tup_cons_expn
-  apply \<phi>reason apply (clarsimp simp add: \<phi>SemType_def subset_iff V_tup_mult \<phi>expns)
-  apply \<phi>reason apply (clarsimp simp add: \<phi>SemType_def subset_iff V_tup_mult \<phi>expns, assumption)
-  apply \<phi>reason apply (clarsimp simp add: \<phi>SemType_def subset_iff V_tup_mult \<phi>expns, assumption)
-  by (rule \<phi>frame0, assumption)
-
-
-
-subsubsection \<open>Accessing Elements\<close>
-
-
-definition op_get_element :: "nat list \<Rightarrow> TY \<Rightarrow> (VAL,'RES_N,'RES) proc"
-  where "op_get_element idx TY =
-    \<phi>M_get_Val (\<lambda>v.
-    \<phi>M_assert (v \<in> Well_Type TY \<and> valid_index TY idx) \<ggreater>
-    \<phi>M_put_Val (index_value idx v))"
-
-definition op_set_element :: "nat list \<Rightarrow> TY \<Rightarrow> (VAL,'RES_N,'RES) proc"
-  where "op_set_element idx TY =
-    \<phi>M_get_Val (\<lambda>u.
-    \<phi>M_get_Val (\<lambda>v.
-    \<phi>M_assert (v \<in> Well_Type TY \<and> valid_index TY idx \<and> u \<in> Well_Type (index_type idx TY)) \<ggreater>
-    \<phi>M_put_Val (index_mod_value idx (\<lambda>_. u) v)
-  ))"
-
-lemma (in \<phi>empty) op_get_element:
-  \<open> \<c>\<o>\<n>\<d>\<i>\<t>\<i>\<o>\<n> valid_index TY idx
-\<Longrightarrow> \<phi>SemType (x \<Ztypecolon> X) TY
-\<Longrightarrow> \<phi>Aggregate_Getter idx X Y f
-\<Longrightarrow> \<p>\<r>\<o>\<c> op_get_element idx TY \<lbrace> VAL x \<Ztypecolon> X \<longmapsto> VAL f x \<Ztypecolon> Y \<rbrace> \<close>
-  unfolding op_get_element_def \<phi>Aggregate_Getter_def Premise_def
-  apply \<phi>reason apply (simp add: \<phi>SemType_def subset_iff)
-  by \<phi>reason
-
-lemma (in \<phi>empty) op_set_element:
-  \<open> \<c>\<o>\<n>\<d>\<i>\<t>\<i>\<o>\<n> valid_index TY idx
-\<Longrightarrow> \<phi>Aggregate_Mapper idx X Y f
-\<Longrightarrow> \<phi>SemType (x \<Ztypecolon> X) TY
-\<Longrightarrow> \<phi>SemType (y \<Ztypecolon> Y) (index_type idx TY)
-\<Longrightarrow> \<p>\<r>\<o>\<c> op_set_element idx TY \<lbrace> VAL x \<Ztypecolon> X\<heavy_comma> VAL y \<Ztypecolon> Y \<longmapsto> f (\<lambda>_. y) x \<Ztypecolon> X \<rbrace>\<close>
-  unfolding op_set_element_def \<phi>Aggregate_Mapper_def Premise_def
-  apply \<phi>reason apply (simp add: \<phi>SemType_def subset_iff)
-   apply (simp add: \<phi>SemType_def subset_iff)
-  by \<phi>reason
-
-
-*)
-
-*)
 
 end
