Phi_Examples/PhiEx_BinTree_AbstModel.thy
@@ -5,6 +5,4 @@ begin
 
 
 
-
-
 end
