Phi_Examples/PhiEx_BinTree_Abstraction.thy
@@ -1,0 +1,5 @@
+theory PhiEx_BinTree_Abstraction
+  imports PhiEx_BinTree_AbstModel
+begin
+
+end
